abp/MediumAutomaton.thy
@@ -3,35 +3,13 @@
  * This file was generated from Medium.maa and will be overridden when changed. To change
  * permanently, consider changing the model itself.
  *
- * Generated on Oct 3, 2018 1:36:23 AM by isartransformer 1.0.0
+ * Generated on Oct 3, 2018 9:18:09 PM by isartransformer 1.0.0
  *)
 theory MediumAutomaton
   imports bundle.tsynBundle automat.ndAutomaton
 
 begin
 
-
-(* TODO Move to tsynStream and find a name for it, the proposed "tsynmap_id" already exists *)
-lemma tsynmap_id_xx[simp]: "tsynDom\<cdot>tsyn \<subseteq> range F \<Longrightarrow> tsynMap F\<cdot>(tsynMap (inv F)\<cdot>tsyn) = tsyn"
-  apply(induction tsyn rule: ind)
-    apply simp_all
-  apply(rename_tac x xs)
-  apply(case_tac x)
-   apply(auto simp add: tsynmap_sconc_msg tsynmap_sconc_null)
-  by(auto simp add: tsyndom_sconc_msg tsyndom_sconc_null f_inv_into_f)
-
-(* TODO: Move to tsynBundle *)
-lemma tsynbundle_ctype: fixes ub::"'m::message tsyn SB"
-  shows "c\<in>ubDom\<cdot>ub \<Longrightarrow> tsynDom\<cdot>(ub . c) \<subseteq> (ctype c)"
-  apply(simp add: tsyndom_insert)
-  using usclOkay_stream_def ctype_tsyn_def
-  by (smt ctype_tsyn_iff mem_Collect_eq subsetCE subsetI ubdom_channel_usokay ubgetch_insert)
-
-(* TODO: Move to UBundle *)
-lemma ub_id_single: "ubDom\<cdot>ub = {c} \<Longrightarrow> Abs_ubundle [c \<mapsto> ub  .  c] = ub"
-  apply(rule ub_eq)
-  apply simp
-  by (simp add: ubWell_single_channel ubdom_ubrep_eq ubgetch_insert)+
 
 (* Helper for easier generation *)
 fun prepend :: "'a::type list \<Rightarrow> 'a \<Rightarrow> 'a list" where
@@ -42,7 +20,7 @@ section \<open>Datatype\<close>
 
 subsection \<open>Definition\<close>
 
-datatype ('e::countable) mediumMessage = DoNotUse_ffb161_MediumE "'e"
+datatype ('e::countable) mediumMessage = DoNotUse_94e0c2_MediumE "'e"
 
 instance mediumMessage :: (countable) countable
   apply(intro_classes)
@@ -52,8 +30,8 @@ instantiation mediumMessage :: (countable) message
 begin
   fun ctype_mediumMessage :: "channel \<Rightarrow> ('e::countable) mediumMessage set" where
   "ctype_mediumMessage c = (
-    if c = \<C> ''DoNotUse_ffb161_ar'' then range DoNotUse_ffb161_MediumE else
-    if c = \<C> ''DoNotUse_ffb161_as'' then range DoNotUse_ffb161_MediumE else
+    if c = \<C> ''DoNotUse_94e0c2_ar'' then range DoNotUse_94e0c2_MediumE else
+    if c = \<C> ''DoNotUse_94e0c2_as'' then range DoNotUse_94e0c2_MediumE else
     undefined)"
   instance
     by(intro_classes)
@@ -63,10 +41,10 @@ end
 subsection \<open>Domain and Range\<close>
 
 definition mediumDom :: "channel set" where
-"mediumDom = {\<C> ''DoNotUse_ffb161_ar''}"
+"mediumDom = {\<C> ''DoNotUse_94e0c2_ar''}"
 
 definition mediumRan :: "channel set" where
-"mediumRan = {\<C> ''DoNotUse_ffb161_as''}"
+"mediumRan = {\<C> ''DoNotUse_94e0c2_as''}"
 
 
 section \<open>Setter\<close>
@@ -75,13 +53,13 @@ subsection \<open>type to sbElem\<close>
 
 (* Do not use this, use mediumElemIn_ar instead *)
 lift_definition mediumElem_raw_ar :: "'e \<Rightarrow> ('e::countable) mediumMessage tsyn sbElem" is
-"\<lambda>x. [\<C> ''DoNotUse_ffb161_ar'' \<mapsto> Msg (DoNotUse_ffb161_MediumE x)]"
+"\<lambda>x. [\<C> ''DoNotUse_94e0c2_ar'' \<mapsto> Msg (DoNotUse_94e0c2_MediumE x)]"
   unfolding sbElemWell_def usclOkay_stream_def ctype_tsyn_def
   by simp
 
 (* Do not use this, use mediumElemOut_as instead *)
 lift_definition mediumElem_raw_as :: "'e \<Rightarrow> ('e::countable) mediumMessage tsyn sbElem" is
-"\<lambda>x. [\<C> ''DoNotUse_ffb161_as'' \<mapsto> Msg (DoNotUse_ffb161_MediumE x)]"
+"\<lambda>x. [\<C> ''DoNotUse_94e0c2_as'' \<mapsto> Msg (DoNotUse_94e0c2_MediumE x)]"
   unfolding sbElemWell_def usclOkay_stream_def ctype_tsyn_def
   by simp
 
@@ -93,12 +71,12 @@ subsubsection \<open>Intern\<close>
 (* Do not use this, use mediumElemIn_ar instead *)
 fun mediumElem_ar :: "'e tsyn \<Rightarrow> ('e::countable) mediumMessage tsyn sbElem" where
 "mediumElem_ar (Msg port_ar) = mediumElem_raw_ar port_ar" |
-"mediumElem_ar null = sbeNull {\<C> ''DoNotUse_ffb161_ar''}"
+"mediumElem_ar null = sbeNull {\<C> ''DoNotUse_94e0c2_ar''}"
 
 (* Do not use this, use mediumElemOut_as instead *)
 fun mediumElem_as :: "'e tsyn \<Rightarrow> ('e::countable) mediumMessage tsyn sbElem" where
 "mediumElem_as (Msg port_as) = mediumElem_raw_as port_as" |
-"mediumElem_as null = sbeNull {\<C> ''DoNotUse_ffb161_as''}"
+"mediumElem_as null = sbeNull {\<C> ''DoNotUse_94e0c2_as''}"
 
 declare mediumElem_ar.simps[simp del]
 
@@ -139,14 +117,14 @@ subsubsection \<open>Intern\<close>
 (* Do not use this, use mediumIn_list_ar instead *)
 fun medium_list_ar :: "('e tsyn) list \<Rightarrow> ('e::countable) mediumMessage tsyn SB" where
 "medium_list_ar (x#xs) = ubConcEq (medium_ar x)\<cdot>(medium_list_ar xs)" |
-"medium_list_ar []     = ubLeast {\<C> ''DoNotUse_ffb161_ar''}"
+"medium_list_ar []     = ubLeast {\<C> ''DoNotUse_94e0c2_ar''}"
 
 declare medium_list_ar.simps[simp del]
 
 (* Do not use this, use mediumOut_list_as instead *)
 fun medium_list_as :: "('e tsyn) list \<Rightarrow> ('e::countable) mediumMessage tsyn SB" where
 "medium_list_as (x#xs) = ubConcEq (medium_as x)\<cdot>(medium_list_as xs)" |
-"medium_list_as []     = ubLeast {\<C> ''DoNotUse_ffb161_as''}"
+"medium_list_as []     = ubLeast {\<C> ''DoNotUse_94e0c2_as''}"
 
 declare medium_list_as.simps[simp del]
 
@@ -168,31 +146,31 @@ subsection \<open>stream to SB\<close>
 
 subsubsection \<open>Intern\<close>
 
-lift_definition DoNotUse_ffb161_medium_stream_ar_h :: "'e tsyn stream \<Rightarrow> ('e::countable) mediumMessage tsyn SB" is
-"\<lambda> s. [(\<C> ''DoNotUse_ffb161_ar'') \<mapsto> (tsynMap (DoNotUse_ffb161_MediumE)\<cdot>s)]"
+lift_definition DoNotUse_94e0c2_medium_stream_ar_h :: "'e tsyn stream \<Rightarrow> ('e::countable) mediumMessage tsyn SB" is
+"\<lambda> s. [(\<C> ''DoNotUse_94e0c2_ar'') \<mapsto> (tsynMap (DoNotUse_94e0c2_MediumE)\<cdot>s)]"
   unfolding ubWell_def usclOkay_stream_def ctype_tsyn_def
   by auto
 
 (* Do not use this, use mediumIn_stream_ar instead *)
 lift_definition medium_stream_ar :: "('e) tsyn stream \<rightarrow> ('e::countable) mediumMessage tsyn SB" is
-"DoNotUse_ffb161_medium_stream_ar_h"
-  apply(auto simp add: cfun_def DoNotUse_ffb161_medium_stream_ar_h_def map_fun_def comp_def)
+"DoNotUse_94e0c2_medium_stream_ar_h"
+  apply(auto simp add: cfun_def DoNotUse_94e0c2_medium_stream_ar_h_def map_fun_def comp_def)
   apply(rule cont_Abs_UB)
   apply(simp add: option_one_cont)
-  by (metis DoNotUse_ffb161_medium_stream_ar_h.rep_eq ubrep_well)
+  by (metis DoNotUse_94e0c2_medium_stream_ar_h.rep_eq ubrep_well)
 
-lift_definition DoNotUse_ffb161_medium_stream_as_h :: "'e tsyn stream \<Rightarrow> ('e::countable) mediumMessage tsyn SB" is
-"\<lambda> s. [(\<C> ''DoNotUse_ffb161_as'') \<mapsto> (tsynMap (DoNotUse_ffb161_MediumE)\<cdot>s)]"
+lift_definition DoNotUse_94e0c2_medium_stream_as_h :: "'e tsyn stream \<Rightarrow> ('e::countable) mediumMessage tsyn SB" is
+"\<lambda> s. [(\<C> ''DoNotUse_94e0c2_as'') \<mapsto> (tsynMap (DoNotUse_94e0c2_MediumE)\<cdot>s)]"
   unfolding ubWell_def usclOkay_stream_def ctype_tsyn_def
   by auto
 
 (* Do not use this, use mediumOut_stream_as instead *)
 lift_definition medium_stream_as :: "('e) tsyn stream \<rightarrow> ('e::countable) mediumMessage tsyn SB" is
-"DoNotUse_ffb161_medium_stream_as_h"
-  apply(auto simp add: cfun_def DoNotUse_ffb161_medium_stream_as_h_def map_fun_def comp_def)
+"DoNotUse_94e0c2_medium_stream_as_h"
+  apply(auto simp add: cfun_def DoNotUse_94e0c2_medium_stream_as_h_def map_fun_def comp_def)
   apply(rule cont_Abs_UB)
   apply(simp add: option_one_cont)
-  by (metis DoNotUse_ffb161_medium_stream_as_h.rep_eq ubrep_well)
+  by (metis DoNotUse_94e0c2_medium_stream_as_h.rep_eq ubrep_well)
 
 
 subsubsection \<open>In/Out\<close>
@@ -210,20 +188,20 @@ section \<open>Getter\<close>
 subsection \<open>sbElem to tsyn\<close>
 
 definition mediumElem_get_ar :: "('e::countable) mediumMessage tsyn sbElem \<Rightarrow> ('e) tsyn" where
-"mediumElem_get_ar sbe = tsynApplyElem (inv DoNotUse_ffb161_MediumE) ((Rep_sbElem sbe) \<rightharpoonup> (\<C> ''DoNotUse_ffb161_ar''))"
+"mediumElem_get_ar sbe = tsynApplyElem (inv DoNotUse_94e0c2_MediumE) ((Rep_sbElem sbe) \<rightharpoonup> (\<C> ''DoNotUse_94e0c2_ar''))"
 
 definition mediumElem_get_as :: "('e::countable) mediumMessage tsyn sbElem \<Rightarrow> ('e) tsyn" where
-"mediumElem_get_as sbe = tsynApplyElem (inv DoNotUse_ffb161_MediumE) ((Rep_sbElem sbe) \<rightharpoonup> (\<C> ''DoNotUse_ffb161_as''))"
+"mediumElem_get_as sbe = tsynApplyElem (inv DoNotUse_94e0c2_MediumE) ((Rep_sbElem sbe) \<rightharpoonup> (\<C> ''DoNotUse_94e0c2_as''))"
 
 
 subsection \<open>SB to stream\<close>
 
 lift_definition medium_get_stream_ar :: "('e::countable) mediumMessage tsyn SB \<rightarrow> 'e tsyn stream" is
-"\<lambda>sb. tsynMap (inv DoNotUse_ffb161_MediumE)\<cdot>(sb . (\<C> ''DoNotUse_ffb161_ar''))"
+"\<lambda>sb. tsynMap (inv DoNotUse_94e0c2_MediumE)\<cdot>(sb . (\<C> ''DoNotUse_94e0c2_ar''))"
   by(simp add: cfun_def)
 
 lift_definition medium_get_stream_as :: "('e::countable) mediumMessage tsyn SB \<rightarrow> 'e tsyn stream" is
-"\<lambda>sb. tsynMap (inv DoNotUse_ffb161_MediumE)\<cdot>(sb . (\<C> ''DoNotUse_ffb161_as''))"
+"\<lambda>sb. tsynMap (inv DoNotUse_94e0c2_MediumE)\<cdot>(sb . (\<C> ''DoNotUse_94e0c2_as''))"
   by(simp add: cfun_def)
 
 
@@ -298,23 +276,23 @@ subsection \<open>tsyn to sbElem/SB\<close>
 
 subsubsection \<open>Intern\<close>
 
-lemma mediumelem_ar_dom[simp]: "sbeDom (mediumElem_ar x) = {\<C> ''DoNotUse_ffb161_ar''}"
+lemma mediumelem_ar_dom[simp]: "sbeDom (mediumElem_ar x) = {\<C> ''DoNotUse_94e0c2_ar''}"
   apply(cases x)
   apply(simp add: mediumElem_ar.simps sbeDom_def mediumElem_raw_ar.rep_eq)
   by(simp add: mediumElem_ar.simps)
 
-lemma mediumelem_as_dom[simp]: "sbeDom (mediumElem_as x) = {\<C> ''DoNotUse_ffb161_as''}"
+lemma mediumelem_as_dom[simp]: "sbeDom (mediumElem_as x) = {\<C> ''DoNotUse_94e0c2_as''}"
   apply(cases x)
   apply(simp add: mediumElem_as.simps sbeDom_def mediumElem_raw_as.rep_eq)
   by(simp add: mediumElem_as.simps)
 
-lemma medium_ar_dom[simp]: "ubDom\<cdot>(medium_ar x) = {\<C> ''DoNotUse_ffb161_ar''}"
+lemma medium_ar_dom[simp]: "ubDom\<cdot>(medium_ar x) = {\<C> ''DoNotUse_94e0c2_ar''}"
   by(simp add: medium_ar_def)
 
 lemma medium_ar_len[simp]: "ubLen (medium_ar x) = 1"
   by(simp add: medium_ar_def)
 
-lemma medium_as_dom[simp]: "ubDom\<cdot>(medium_as x) = {\<C> ''DoNotUse_ffb161_as''}"
+lemma medium_as_dom[simp]: "ubDom\<cdot>(medium_as x) = {\<C> ''DoNotUse_94e0c2_as''}"
   by(simp add: medium_as_def)
 
 lemma medium_as_len[simp]: "ubLen (medium_as x) = 1"
@@ -346,41 +324,41 @@ subsection \<open>stream to SB\<close>
 
 subsubsection \<open>Intern\<close>
 
-lemma medium_stream_ar_dom[simp]: "ubDom\<cdot>(medium_stream_ar\<cdot>x) = {\<C> ''DoNotUse_ffb161_ar''}"
-  by(simp add: medium_stream_ar.rep_eq ubdom_insert DoNotUse_ffb161_medium_stream_ar_h.rep_eq)
+lemma medium_stream_ar_dom[simp]: "ubDom\<cdot>(medium_stream_ar\<cdot>x) = {\<C> ''DoNotUse_94e0c2_ar''}"
+  by(simp add: medium_stream_ar.rep_eq ubdom_insert DoNotUse_94e0c2_medium_stream_ar_h.rep_eq)
 
 lemma medium_stream_ar_len[simp]: "ubLen (medium_stream_ar\<cdot>x) = #x"
   apply(subst uslen_ubLen_ch3)
   apply simp
   apply(simp add: medium_stream_ar.rep_eq)
-  apply(simp add: ubGetCh_def DoNotUse_ffb161_medium_stream_ar_h.rep_eq)
+  apply(simp add: ubGetCh_def DoNotUse_94e0c2_medium_stream_ar_h.rep_eq)
   by (simp add: tsynmap_slen usclLen_stream_def)
 
 lemma medium_stream_ar_id[simp]:
-  assumes "ubDom\<cdot>ub = {\<C> ''DoNotUse_ffb161_ar''} "
+  assumes "ubDom\<cdot>ub = {\<C> ''DoNotUse_94e0c2_ar''} "
     shows "medium_stream_ar\<cdot>(medium_get_stream_ar\<cdot>ub) = ub"
   apply(simp add: medium_stream_ar.rep_eq medium_get_stream_ar.rep_eq)
-  apply(simp add: DoNotUse_ffb161_medium_stream_ar_h_def)
-  apply(subst tsynmap_id_xx)
+  apply(simp add: DoNotUse_94e0c2_medium_stream_ar_h_def)
+  apply(subst tsynmap_inv_id)
   using assms tsynbundle_ctype apply fastforce
   using assms ub_id_single by blast
 
-lemma medium_stream_as_dom[simp]: "ubDom\<cdot>(medium_stream_as\<cdot>x) = {\<C> ''DoNotUse_ffb161_as''}"
-  by(simp add: medium_stream_as.rep_eq ubdom_insert DoNotUse_ffb161_medium_stream_as_h.rep_eq)
+lemma medium_stream_as_dom[simp]: "ubDom\<cdot>(medium_stream_as\<cdot>x) = {\<C> ''DoNotUse_94e0c2_as''}"
+  by(simp add: medium_stream_as.rep_eq ubdom_insert DoNotUse_94e0c2_medium_stream_as_h.rep_eq)
 
 lemma medium_stream_as_len[simp]: "ubLen (medium_stream_as\<cdot>x) = #x"
   apply(subst uslen_ubLen_ch3)
   apply simp
   apply(simp add: medium_stream_as.rep_eq)
-  apply(simp add: ubGetCh_def DoNotUse_ffb161_medium_stream_as_h.rep_eq)
+  apply(simp add: ubGetCh_def DoNotUse_94e0c2_medium_stream_as_h.rep_eq)
   by (simp add: tsynmap_slen usclLen_stream_def)
 
 lemma medium_stream_as_id[simp]:
-  assumes "ubDom\<cdot>ub = {\<C> ''DoNotUse_ffb161_as''} "
+  assumes "ubDom\<cdot>ub = {\<C> ''DoNotUse_94e0c2_as''} "
     shows "medium_stream_as\<cdot>(medium_get_stream_as\<cdot>ub) = ub"
   apply(simp add: medium_stream_as.rep_eq medium_get_stream_as.rep_eq)
-  apply(simp add: DoNotUse_ffb161_medium_stream_as_h_def)
-  apply(subst tsynmap_id_xx)
+  apply(simp add: DoNotUse_94e0c2_medium_stream_as_h_def)
+  apply(subst tsynmap_inv_id)
   using assms tsynbundle_ctype apply fastforce
   using assms ub_id_single by blast
 
@@ -402,7 +380,7 @@ subsection \<open>sbElem to tsyn\<close>
 
 subsubsection \<open>Intern\<close>
 
-lemma mediumelem_ar_id[simp]: "mediumElem_get_ar (mediumElem_ar x) = x"
+lemma mediumelem_get_ar_id[simp]: "mediumElem_get_ar (mediumElem_ar x) = x"
   apply(cases x)
   apply(auto simp add: mediumElem_ar.simps)
   unfolding mediumElem_get_ar_def mediumElem_raw_ar.rep_eq
@@ -410,7 +388,7 @@ lemma mediumelem_ar_id[simp]: "mediumElem_get_ar (mediumElem_ar x) = x"
   apply (meson f_inv_into_f rangeI mediumMessage.inject)
   by(simp add: sbeNull.rep_eq)
 
-lemma mediumelem_as_id[simp]: "mediumElem_get_as (mediumElem_as x) = x"
+lemma mediumelem_get_as_id[simp]: "mediumElem_get_as (mediumElem_as x) = x"
   apply(cases x)
   apply(auto simp add: mediumElem_as.simps)
   unfolding mediumElem_get_as_def mediumElem_raw_as.rep_eq
@@ -421,46 +399,93 @@ lemma mediumelem_as_id[simp]: "mediumElem_get_as (mediumElem_as x) = x"
 
 subsubsection \<open>In/Out\<close>
 
-lemma mediumelemin_ar_ar_id[simp]: "mediumElem_get_ar (mediumElemIn_ar port_ar) = port_ar"
+lemma mediumelem_get_ar_in_ar_id[simp]: "mediumElem_get_ar (mediumElemIn_ar port_ar) = port_ar"
   apply(simp add: mediumElemIn_ar_def mediumElem_get_ar_def)
-  by(metis mediumElem_get_ar_def mediumelem_ar_id)
+  by(metis mediumElem_get_ar_def mediumelem_get_ar_id)
 
-lemma mediumelemout_as_as_id[simp]: "mediumElem_get_as (mediumElemOut_as port_as) = port_as"
+lemma mediumelem_get_as_out_as_id[simp]: "mediumElem_get_as (mediumElemOut_as port_as) = port_as"
   apply(simp add: mediumElemOut_as_def mediumElem_get_as_def)
-  by(metis mediumElem_get_as_def mediumelem_as_id)
+  by(metis mediumElem_get_as_def mediumelem_get_as_id)
 
 
 subsection \<open>SB to stream\<close>
 
 subsubsection \<open>Intern\<close>
 
-lemma medium_stream_ar_id[simp]: "medium_get_stream_ar\<cdot>(medium_stream_ar\<cdot>x) = x"
+lemma medium_get_stream_ar_id[simp]: "medium_get_stream_ar\<cdot>(medium_stream_ar\<cdot>x) = x"
   apply(simp add: medium_get_stream_ar.rep_eq medium_stream_ar.rep_eq)
-  apply(simp add: ubGetCh_def DoNotUse_ffb161_medium_stream_ar_h.rep_eq)
+  apply(simp add: ubGetCh_def DoNotUse_94e0c2_medium_stream_ar_h.rep_eq)
   by (simp add: inj_def)
 
-lemma medium_stream_as_id[simp]: "medium_get_stream_as\<cdot>(medium_stream_as\<cdot>x) = x"
+lemma medium_get_stream_ar_eq:
+  assumes "ubDom\<cdot>ub1 = {\<C> ''DoNotUse_94e0c2_ar''}"
+      and "ubDom\<cdot>ub2 = {\<C> ''DoNotUse_94e0c2_ar''}"
+      and "medium_get_stream_ar\<cdot>ub1 = medium_get_stream_ar\<cdot>ub2"
+    shows "ub1 = ub2"
+  (* TODO Doesnt work for non-generic ABPComponent *)
+  (*using assms(1) assms(2) assms(3) medium_stream_ar_id by fastforce*)
+  sorry
+
+lemma medium_get_stream_ar_conc[simp]:
+  assumes "\<C> ''DoNotUse_94e0c2_ar'' \<in> ubDom\<cdot>ub1"
+      and "\<C> ''DoNotUse_94e0c2_ar'' \<in> ubDom\<cdot>ub2"
+    shows "medium_get_stream_ar\<cdot>(ubConc ub1\<cdot>ub2) = (medium_get_stream_ar\<cdot>ub1) \<bullet> (medium_get_stream_ar\<cdot>ub2)"
+  apply(simp add: medium_get_stream_ar.rep_eq)
+  apply (subst ubConc_usclConc_eq)
+  using assms(1) apply blast
+  using assms(2) apply blast
+  by (simp add: tsynmap_sconc usclConc_stream_def)
+
+lemma medium_get_stream_as_id[simp]: "medium_get_stream_as\<cdot>(medium_stream_as\<cdot>x) = x"
   apply(simp add: medium_get_stream_as.rep_eq medium_stream_as.rep_eq)
-  apply(simp add: ubGetCh_def DoNotUse_ffb161_medium_stream_as_h.rep_eq)
+  apply(simp add: ubGetCh_def DoNotUse_94e0c2_medium_stream_as_h.rep_eq)
   by (simp add: inj_def)
+
+lemma medium_get_stream_as_eq:
+  assumes "ubDom\<cdot>ub1 = {\<C> ''DoNotUse_94e0c2_as''}"
+      and "ubDom\<cdot>ub2 = {\<C> ''DoNotUse_94e0c2_as''}"
+      and "medium_get_stream_as\<cdot>ub1 = medium_get_stream_as\<cdot>ub2"
+    shows "ub1 = ub2"
+  (* TODO Doesnt work for non-generic ABPComponent *)
+  (*using assms(1) assms(2) assms(3) medium_stream_as_id by fastforce*)
+  sorry
+
+lemma medium_get_stream_as_conc[simp]:
+  assumes "\<C> ''DoNotUse_94e0c2_as'' \<in> ubDom\<cdot>ub1"
+      and "\<C> ''DoNotUse_94e0c2_as'' \<in> ubDom\<cdot>ub2"
+    shows "medium_get_stream_as\<cdot>(ubConc ub1\<cdot>ub2) = (medium_get_stream_as\<cdot>ub1) \<bullet> (medium_get_stream_as\<cdot>ub2)"
+  apply(simp add: medium_get_stream_as.rep_eq)
+  apply (subst ubConc_usclConc_eq)
+  using assms(1) apply blast
+  using assms(2) apply blast
+  by (simp add: tsynmap_sconc usclConc_stream_def)
 
 
 subsubsection \<open>In/Out\<close>
 
-lemma mediumin_stream_ar_ar_id[simp]: "medium_get_stream_ar\<cdot>(mediumIn_stream_ar\<cdot>port_ar) = port_ar"
+lemma medium_get_stream_ar_in_ar_id[simp]: "medium_get_stream_ar\<cdot>(mediumIn_stream_ar\<cdot>port_ar) = port_ar"
   apply(auto simp add: medium_get_stream_ar.rep_eq mediumIn_stream_ar_def ubclUnion_ubundle_def)
-  by (metis medium_get_stream_ar.rep_eq medium_stream_ar_id)
+  by (metis medium_get_stream_ar.rep_eq medium_get_stream_ar_id)
 
-lemma mediumout_stream_as_as_id[simp]: "medium_get_stream_as\<cdot>(mediumOut_stream_as\<cdot>port_as) = port_as"
+lemma medium_get_stream_as_out_as_id[simp]: "medium_get_stream_as\<cdot>(mediumOut_stream_as\<cdot>port_as) = port_as"
   apply(auto simp add: medium_get_stream_as.rep_eq mediumOut_stream_as_def ubclUnion_ubundle_def)
-  by (metis medium_get_stream_as.rep_eq medium_stream_as_id)
+  by (metis medium_get_stream_as.rep_eq medium_get_stream_as_id)
 
 
 subsection \<open>tsyn to SB to one-element stream\<close>
 
+subsubsection \<open>Intern\<close>
+
+lemma medium_get_stream_ar_single[simp]: "medium_get_stream_ar\<cdot>(medium_ar x) = \<up>x"
+  sorry
+
+lemma medium_get_stream_as_single[simp]: "medium_get_stream_as\<cdot>(medium_as x) = \<up>x"
+  sorry
+
+
 subsubsection \<open>In/Out\<close>
 
-lemma mediumin_ar_ar_id[simp]: "medium_get_stream_ar\<cdot>(mediumIn_ar port_ar) = \<up>port_ar"
+lemma medium_get_stream_ar_single_in_ar_id[simp]: "medium_get_stream_ar\<cdot>(mediumIn_ar port_ar) = \<up>port_ar"
   apply(simp add: medium_get_stream_ar_def mediumIn_ar_def)
   apply(subst sbe2sb_getch)
   apply(auto simp add: mediumDom_def mediumElemIn_ar_def)
@@ -470,7 +495,7 @@ lemma mediumin_ar_ar_id[simp]: "medium_get_stream_ar\<cdot>(mediumIn_ar port_ar)
   apply(simp add: inj_def)
   by(simp add: sbeNull.rep_eq)
 
-lemma mediumout_as_as_id[simp]: "medium_get_stream_as\<cdot>(mediumOut_as port_as) = \<up>port_as"
+lemma medium_get_stream_as_single_out_as_id[simp]: "medium_get_stream_as\<cdot>(mediumOut_as port_as) = \<up>port_as"
   apply(simp add: medium_get_stream_as_def mediumOut_as_def)
   apply(subst sbe2sb_getch)
   apply(auto simp add: mediumDom_def mediumElemOut_as_def)
@@ -479,6 +504,23 @@ lemma mediumout_as_as_id[simp]: "medium_get_stream_as\<cdot>(mediumOut_as port_a
   unfolding mediumElem_get_as_def mediumElem_raw_as.rep_eq
   apply(simp add: inj_def)
   by(simp add: sbeNull.rep_eq)
+
+
+section \<open>More Setter-Lemmas\<close>
+
+subsection \<open>SB to stream\<close>
+
+subsubsection \<open>Intern\<close>
+
+lemma medium_stream_ar_conc:
+  "medium_stream_ar\<cdot>(\<up>elem \<bullet> s) = ubConc (medium_ar elem)\<cdot>(medium_stream_ar\<cdot>s)"
+  apply (rule medium_get_stream_ar_eq)
+  by simp_all
+
+lemma medium_stream_as_conc:
+  "medium_stream_as\<cdot>(\<up>elem \<bullet> s) = ubConc (medium_as elem)\<cdot>(medium_stream_as\<cdot>s)"
+  apply (rule medium_get_stream_as_eq)
+  by simp_all
 
 
 section \<open>Step-wise lemmata for the transition function\<close>
