abp/ReceiverAutomaton.thy
@@ -3,35 +3,13 @@
  * This file was generated from Receiver.maa and will be overridden when changed. To change
  * permanently, consider changing the model itself.
  *
- * Generated on Oct 3, 2018 1:36:21 AM by isartransformer 1.0.0
+ * Generated on Oct 3, 2018 9:18:08 PM by isartransformer 1.0.0
  *)
 theory ReceiverAutomaton
   imports bundle.tsynBundle automat.dAutomaton
 
 begin
 
-
-(* TODO Move to tsynStream and find a name for it, the proposed "tsynmap_id" already exists *)
-lemma tsynmap_id_xx[simp]: "tsynDom\<cdot>tsyn \<subseteq> range F \<Longrightarrow> tsynMap (F \<circ> (inv F))\<cdot>tsyn = tsyn"
-  apply(induction tsyn rule: ind)
-    apply simp_all
-  apply(rename_tac x xs)
-  apply(case_tac x)
-   apply(auto simp add: tsynmap_sconc_msg tsynmap_sconc_null)
-  by(auto simp add: tsyndom_sconc_msg tsyndom_sconc_null f_inv_into_f)
-
-(* TODO: Move to tsynBundle *)
-lemma tsynbundle_ctype: fixes ub::"'m::message tsyn SB"
-  shows "c\<in>ubDom\<cdot>ub \<Longrightarrow> tsynDom\<cdot>(ub . c) \<subseteq> (ctype c)"
-  apply(simp add: tsyndom_insert)
-  using usclOkay_stream_def ctype_tsyn_def
-  by (smt ctype_tsyn_iff mem_Collect_eq subsetCE subsetI ubdom_channel_usokay ubgetch_insert)
-
-(* TODO: Move to UBundle *)
-lemma ub_id_single: "ubDom\<cdot>ub = {c} \<Longrightarrow> Abs_ubundle [c \<mapsto> ub  .  c] = ub"
-  apply(rule ub_eq)
-  apply simp
-  by (simp add: ubWell_single_channel ubdom_ubrep_eq ubgetch_insert)+
 
 (* Helper for easier generation *)
 fun prepend :: "'a::type list \<Rightarrow> 'a \<Rightarrow> 'a list" where
@@ -42,7 +20,7 @@ section \<open>Datatype\<close>
 
 subsection \<open>Definition\<close>
 
-datatype ('e::countable) receiverMessage = DoNotUse_277815_ReceiverPair_E_Bool "('e\<times>bool)" | DoNotUse_277815_ReceiverBool "bool" | DoNotUse_277815_ReceiverE "'e"
+datatype ('e::countable) receiverMessage = DoNotUse_5cf0af_ReceiverPair_E_Bool "('e\<times>bool)" | DoNotUse_5cf0af_ReceiverBool "bool" | DoNotUse_5cf0af_ReceiverE "'e"
 
 instance receiverMessage :: (countable) countable
   apply(intro_classes)
@@ -52,9 +30,9 @@ instantiation receiverMessage :: (countable) message
 begin
   fun ctype_receiverMessage :: "channel \<Rightarrow> ('e::countable) receiverMessage set" where
   "ctype_receiverMessage c = (
-    if c = \<C> ''DoNotUse_277815_dr'' then range DoNotUse_277815_ReceiverPair_E_Bool else
-    if c = \<C> ''DoNotUse_277815_ar'' then range DoNotUse_277815_ReceiverBool else
-    if c = \<C> ''DoNotUse_277815_o'' then range DoNotUse_277815_ReceiverE else
+    if c = \<C> ''DoNotUse_5cf0af_dr'' then range DoNotUse_5cf0af_ReceiverPair_E_Bool else
+    if c = \<C> ''DoNotUse_5cf0af_ar'' then range DoNotUse_5cf0af_ReceiverBool else
+    if c = \<C> ''DoNotUse_5cf0af_o'' then range DoNotUse_5cf0af_ReceiverE else
     undefined)"
   instance
     by(intro_classes)
@@ -64,10 +42,10 @@ end
 subsection \<open>Domain and Range\<close>
 
 definition receiverDom :: "channel set" where
-"receiverDom = {\<C> ''DoNotUse_277815_dr''}"
+"receiverDom = {\<C> ''DoNotUse_5cf0af_dr''}"
 
 definition receiverRan :: "channel set" where
-"receiverRan = {\<C> ''DoNotUse_277815_ar'', \<C> ''DoNotUse_277815_o''}"
+"receiverRan = {\<C> ''DoNotUse_5cf0af_ar'', \<C> ''DoNotUse_5cf0af_o''}"
 
 
 section \<open>Setter\<close>
@@ -76,19 +54,19 @@ subsection \<open>type to sbElem\<close>
 
 (* Do not use this, use receiverElemIn_dr instead *)
 lift_definition receiverElem_raw_dr :: "('e\<times>bool) \<Rightarrow> ('e::countable) receiverMessage tsyn sbElem" is
-"\<lambda>x. [\<C> ''DoNotUse_277815_dr'' \<mapsto> Msg (DoNotUse_277815_ReceiverPair_E_Bool x)]"
+"\<lambda>x. [\<C> ''DoNotUse_5cf0af_dr'' \<mapsto> Msg (DoNotUse_5cf0af_ReceiverPair_E_Bool x)]"
   unfolding sbElemWell_def usclOkay_stream_def ctype_tsyn_def
   by simp
 
 (* Do not use this, use receiverElemOut_ar_o instead *)
 lift_definition receiverElem_raw_ar :: "bool \<Rightarrow> ('e::countable) receiverMessage tsyn sbElem" is
-"\<lambda>x. [\<C> ''DoNotUse_277815_ar'' \<mapsto> Msg (DoNotUse_277815_ReceiverBool x)]"
+"\<lambda>x. [\<C> ''DoNotUse_5cf0af_ar'' \<mapsto> Msg (DoNotUse_5cf0af_ReceiverBool x)]"
   unfolding sbElemWell_def usclOkay_stream_def ctype_tsyn_def
   by simp
 
 (* Do not use this, use receiverElemOut_ar_o instead *)
 lift_definition receiverElem_raw_o :: "'e \<Rightarrow> ('e::countable) receiverMessage tsyn sbElem" is
-"\<lambda>x. [\<C> ''DoNotUse_277815_o'' \<mapsto> Msg (DoNotUse_277815_ReceiverE x)]"
+"\<lambda>x. [\<C> ''DoNotUse_5cf0af_o'' \<mapsto> Msg (DoNotUse_5cf0af_ReceiverE x)]"
   unfolding sbElemWell_def usclOkay_stream_def ctype_tsyn_def
   by simp
 
@@ -100,17 +78,17 @@ subsubsection \<open>Intern\<close>
 (* Do not use this, use receiverElemIn_dr instead *)
 fun receiverElem_dr :: "('e\<times>bool) tsyn \<Rightarrow> ('e::countable) receiverMessage tsyn sbElem" where
 "receiverElem_dr (Msg port_dr) = receiverElem_raw_dr port_dr" |
-"receiverElem_dr null = sbeNull {\<C> ''DoNotUse_277815_dr''}"
+"receiverElem_dr null = sbeNull {\<C> ''DoNotUse_5cf0af_dr''}"
 
 (* Do not use this, use receiverElemOut_ar_o instead *)
 fun receiverElem_ar :: "bool tsyn \<Rightarrow> ('e::countable) receiverMessage tsyn sbElem" where
 "receiverElem_ar (Msg port_ar) = receiverElem_raw_ar port_ar" |
-"receiverElem_ar null = sbeNull {\<C> ''DoNotUse_277815_ar''}"
+"receiverElem_ar null = sbeNull {\<C> ''DoNotUse_5cf0af_ar''}"
 
 (* Do not use this, use receiverElemOut_ar_o instead *)
 fun receiverElem_o :: "'e tsyn \<Rightarrow> ('e::countable) receiverMessage tsyn sbElem" where
 "receiverElem_o (Msg port_o) = receiverElem_raw_o port_o" |
-"receiverElem_o null = sbeNull {\<C> ''DoNotUse_277815_o''}"
+"receiverElem_o null = sbeNull {\<C> ''DoNotUse_5cf0af_o''}"
 
 declare receiverElem_dr.simps[simp del]
 
@@ -157,21 +135,21 @@ subsubsection \<open>Intern\<close>
 (* Do not use this, use receiverIn_list_dr instead *)
 fun receiver_list_dr :: "(('e\<times>bool) tsyn) list \<Rightarrow> ('e::countable) receiverMessage tsyn SB" where
 "receiver_list_dr (x#xs) = ubConcEq (receiver_dr x)\<cdot>(receiver_list_dr xs)" |
-"receiver_list_dr []     = ubLeast {\<C> ''DoNotUse_277815_dr''}"
+"receiver_list_dr []     = ubLeast {\<C> ''DoNotUse_5cf0af_dr''}"
 
 declare receiver_list_dr.simps[simp del]
 
 (* Do not use this, use receiverOut_list_ar_o instead *)
 fun receiver_list_ar :: "(bool tsyn) list \<Rightarrow> ('e::countable) receiverMessage tsyn SB" where
 "receiver_list_ar (x#xs) = ubConcEq (receiver_ar x)\<cdot>(receiver_list_ar xs)" |
-"receiver_list_ar []     = ubLeast {\<C> ''DoNotUse_277815_ar''}"
+"receiver_list_ar []     = ubLeast {\<C> ''DoNotUse_5cf0af_ar''}"
 
 declare receiver_list_ar.simps[simp del]
 
 (* Do not use this, use receiverOut_list_ar_o instead *)
 fun receiver_list_o :: "('e tsyn) list \<Rightarrow> ('e::countable) receiverMessage tsyn SB" where
 "receiver_list_o (x#xs) = ubConcEq (receiver_o x)\<cdot>(receiver_list_o xs)" |
-"receiver_list_o []     = ubLeast {\<C> ''DoNotUse_277815_o''}"
+"receiver_list_o []     = ubLeast {\<C> ''DoNotUse_5cf0af_o''}"
 
 declare receiver_list_o.simps[simp del]
 
@@ -193,44 +171,44 @@ subsection \<open>stream to SB\<close>
 
 subsubsection \<open>Intern\<close>
 
-lift_definition DoNotUse_277815_receiver_stream_dr_h :: "('e\<times>bool) tsyn stream \<Rightarrow> ('e::countable) receiverMessage tsyn SB" is
-"\<lambda> s. [(\<C> ''DoNotUse_277815_dr'') \<mapsto> (tsynMap (DoNotUse_277815_ReceiverPair_E_Bool)\<cdot>s)]"
+lift_definition DoNotUse_5cf0af_receiver_stream_dr_h :: "('e\<times>bool) tsyn stream \<Rightarrow> ('e::countable) receiverMessage tsyn SB" is
+"\<lambda> s. [(\<C> ''DoNotUse_5cf0af_dr'') \<mapsto> (tsynMap (DoNotUse_5cf0af_ReceiverPair_E_Bool)\<cdot>s)]"
   unfolding ubWell_def usclOkay_stream_def ctype_tsyn_def
   by auto
 
 (* Do not use this, use receiverIn_stream_dr instead *)
 lift_definition receiver_stream_dr :: "(('e\<times>bool)) tsyn stream \<rightarrow> ('e::countable) receiverMessage tsyn SB" is
-"DoNotUse_277815_receiver_stream_dr_h"
-  apply(auto simp add: cfun_def DoNotUse_277815_receiver_stream_dr_h_def map_fun_def comp_def)
+"DoNotUse_5cf0af_receiver_stream_dr_h"
+  apply(auto simp add: cfun_def DoNotUse_5cf0af_receiver_stream_dr_h_def map_fun_def comp_def)
   apply(rule cont_Abs_UB)
   apply(simp add: option_one_cont)
-  by (metis DoNotUse_277815_receiver_stream_dr_h.rep_eq ubrep_well)
+  by (metis DoNotUse_5cf0af_receiver_stream_dr_h.rep_eq ubrep_well)
 
-lift_definition DoNotUse_277815_receiver_stream_ar_h :: "bool tsyn stream \<Rightarrow> ('e::countable) receiverMessage tsyn SB" is
-"\<lambda> s. [(\<C> ''DoNotUse_277815_ar'') \<mapsto> (tsynMap (DoNotUse_277815_ReceiverBool)\<cdot>s)]"
+lift_definition DoNotUse_5cf0af_receiver_stream_ar_h :: "bool tsyn stream \<Rightarrow> ('e::countable) receiverMessage tsyn SB" is
+"\<lambda> s. [(\<C> ''DoNotUse_5cf0af_ar'') \<mapsto> (tsynMap (DoNotUse_5cf0af_ReceiverBool)\<cdot>s)]"
   unfolding ubWell_def usclOkay_stream_def ctype_tsyn_def
   by auto
 
 (* Do not use this, use receiverOut_stream_ar_o instead *)
 lift_definition receiver_stream_ar :: "(bool) tsyn stream \<rightarrow> ('e::countable) receiverMessage tsyn SB" is
-"DoNotUse_277815_receiver_stream_ar_h"
-  apply(auto simp add: cfun_def DoNotUse_277815_receiver_stream_ar_h_def map_fun_def comp_def)
+"DoNotUse_5cf0af_receiver_stream_ar_h"
+  apply(auto simp add: cfun_def DoNotUse_5cf0af_receiver_stream_ar_h_def map_fun_def comp_def)
   apply(rule cont_Abs_UB)
   apply(simp add: option_one_cont)
-  by (metis DoNotUse_277815_receiver_stream_ar_h.rep_eq ubrep_well)
+  by (metis DoNotUse_5cf0af_receiver_stream_ar_h.rep_eq ubrep_well)
 
-lift_definition DoNotUse_277815_receiver_stream_o_h :: "'e tsyn stream \<Rightarrow> ('e::countable) receiverMessage tsyn SB" is
-"\<lambda> s. [(\<C> ''DoNotUse_277815_o'') \<mapsto> (tsynMap (DoNotUse_277815_ReceiverE)\<cdot>s)]"
+lift_definition DoNotUse_5cf0af_receiver_stream_o_h :: "'e tsyn stream \<Rightarrow> ('e::countable) receiverMessage tsyn SB" is
+"\<lambda> s. [(\<C> ''DoNotUse_5cf0af_o'') \<mapsto> (tsynMap (DoNotUse_5cf0af_ReceiverE)\<cdot>s)]"
   unfolding ubWell_def usclOkay_stream_def ctype_tsyn_def
   by auto
 
 (* Do not use this, use receiverOut_stream_ar_o instead *)
 lift_definition receiver_stream_o :: "('e) tsyn stream \<rightarrow> ('e::countable) receiverMessage tsyn SB" is
-"DoNotUse_277815_receiver_stream_o_h"
-  apply(auto simp add: cfun_def DoNotUse_277815_receiver_stream_o_h_def map_fun_def comp_def)
+"DoNotUse_5cf0af_receiver_stream_o_h"
+  apply(auto simp add: cfun_def DoNotUse_5cf0af_receiver_stream_o_h_def map_fun_def comp_def)
   apply(rule cont_Abs_UB)
   apply(simp add: option_one_cont)
-  by (metis DoNotUse_277815_receiver_stream_o_h.rep_eq ubrep_well)
+  by (metis DoNotUse_5cf0af_receiver_stream_o_h.rep_eq ubrep_well)
 
 
 subsubsection \<open>In/Out\<close>
@@ -248,27 +226,27 @@ section \<open>Getter\<close>
 subsection \<open>sbElem to tsyn\<close>
 
 definition receiverElem_get_dr :: "('e::countable) receiverMessage tsyn sbElem \<Rightarrow> (('e\<times>bool)) tsyn" where
-"receiverElem_get_dr sbe = tsynApplyElem (inv DoNotUse_277815_ReceiverPair_E_Bool) ((Rep_sbElem sbe) \<rightharpoonup> (\<C> ''DoNotUse_277815_dr''))"
+"receiverElem_get_dr sbe = tsynApplyElem (inv DoNotUse_5cf0af_ReceiverPair_E_Bool) ((Rep_sbElem sbe) \<rightharpoonup> (\<C> ''DoNotUse_5cf0af_dr''))"
 
 definition receiverElem_get_ar :: "('e::countable) receiverMessage tsyn sbElem \<Rightarrow> (bool) tsyn" where
-"receiverElem_get_ar sbe = tsynApplyElem (inv DoNotUse_277815_ReceiverBool) ((Rep_sbElem sbe) \<rightharpoonup> (\<C> ''DoNotUse_277815_ar''))"
+"receiverElem_get_ar sbe = tsynApplyElem (inv DoNotUse_5cf0af_ReceiverBool) ((Rep_sbElem sbe) \<rightharpoonup> (\<C> ''DoNotUse_5cf0af_ar''))"
 
 definition receiverElem_get_o :: "('e::countable) receiverMessage tsyn sbElem \<Rightarrow> ('e) tsyn" where
-"receiverElem_get_o sbe = tsynApplyElem (inv DoNotUse_277815_ReceiverE) ((Rep_sbElem sbe) \<rightharpoonup> (\<C> ''DoNotUse_277815_o''))"
+"receiverElem_get_o sbe = tsynApplyElem (inv DoNotUse_5cf0af_ReceiverE) ((Rep_sbElem sbe) \<rightharpoonup> (\<C> ''DoNotUse_5cf0af_o''))"
 
 
 subsection \<open>SB to stream\<close>
 
 lift_definition receiver_get_stream_dr :: "('e::countable) receiverMessage tsyn SB \<rightarrow> ('e\<times>bool) tsyn stream" is
-"\<lambda>sb. tsynMap (inv DoNotUse_277815_ReceiverPair_E_Bool)\<cdot>(sb . (\<C> ''DoNotUse_277815_dr''))"
+"\<lambda>sb. tsynMap (inv DoNotUse_5cf0af_ReceiverPair_E_Bool)\<cdot>(sb . (\<C> ''DoNotUse_5cf0af_dr''))"
   by(simp add: cfun_def)
 
 lift_definition receiver_get_stream_ar :: "('e::countable) receiverMessage tsyn SB \<rightarrow> bool tsyn stream" is
-"\<lambda>sb. tsynMap (inv DoNotUse_277815_ReceiverBool)\<cdot>(sb . (\<C> ''DoNotUse_277815_ar''))"
+"\<lambda>sb. tsynMap (inv DoNotUse_5cf0af_ReceiverBool)\<cdot>(sb . (\<C> ''DoNotUse_5cf0af_ar''))"
   by(simp add: cfun_def)
 
 lift_definition receiver_get_stream_o :: "('e::countable) receiverMessage tsyn SB \<rightarrow> 'e tsyn stream" is
-"\<lambda>sb. tsynMap (inv DoNotUse_277815_ReceiverE)\<cdot>(sb . (\<C> ''DoNotUse_277815_o''))"
+"\<lambda>sb. tsynMap (inv DoNotUse_5cf0af_ReceiverE)\<cdot>(sb . (\<C> ''DoNotUse_5cf0af_o''))"
   by(simp add: cfun_def)
 
 
@@ -357,34 +335,34 @@ subsection \<open>tsyn to sbElem/SB\<close>
 
 subsubsection \<open>Intern\<close>
 
-lemma receiverelem_dr_dom[simp]: "sbeDom (receiverElem_dr x) = {\<C> ''DoNotUse_277815_dr''}"
+lemma receiverelem_dr_dom[simp]: "sbeDom (receiverElem_dr x) = {\<C> ''DoNotUse_5cf0af_dr''}"
   apply(cases x)
   apply(simp add: receiverElem_dr.simps sbeDom_def receiverElem_raw_dr.rep_eq)
   by(simp add: receiverElem_dr.simps)
 
-lemma receiverelem_ar_dom[simp]: "sbeDom (receiverElem_ar x) = {\<C> ''DoNotUse_277815_ar''}"
+lemma receiverelem_ar_dom[simp]: "sbeDom (receiverElem_ar x) = {\<C> ''DoNotUse_5cf0af_ar''}"
   apply(cases x)
   apply(simp add: receiverElem_ar.simps sbeDom_def receiverElem_raw_ar.rep_eq)
   by(simp add: receiverElem_ar.simps)
 
-lemma receiverelem_o_dom[simp]: "sbeDom (receiverElem_o x) = {\<C> ''DoNotUse_277815_o''}"
+lemma receiverelem_o_dom[simp]: "sbeDom (receiverElem_o x) = {\<C> ''DoNotUse_5cf0af_o''}"
   apply(cases x)
   apply(simp add: receiverElem_o.simps sbeDom_def receiverElem_raw_o.rep_eq)
   by(simp add: receiverElem_o.simps)
 
-lemma receiver_dr_dom[simp]: "ubDom\<cdot>(receiver_dr x) = {\<C> ''DoNotUse_277815_dr''}"
+lemma receiver_dr_dom[simp]: "ubDom\<cdot>(receiver_dr x) = {\<C> ''DoNotUse_5cf0af_dr''}"
   by(simp add: receiver_dr_def)
 
 lemma receiver_dr_len[simp]: "ubLen (receiver_dr x) = 1"
   by(simp add: receiver_dr_def)
 
-lemma receiver_ar_dom[simp]: "ubDom\<cdot>(receiver_ar x) = {\<C> ''DoNotUse_277815_ar''}"
+lemma receiver_ar_dom[simp]: "ubDom\<cdot>(receiver_ar x) = {\<C> ''DoNotUse_5cf0af_ar''}"
   by(simp add: receiver_ar_def)
 
 lemma receiver_ar_len[simp]: "ubLen (receiver_ar x) = 1"
   by(simp add: receiver_ar_def)
 
-lemma receiver_o_dom[simp]: "ubDom\<cdot>(receiver_o x) = {\<C> ''DoNotUse_277815_o''}"
+lemma receiver_o_dom[simp]: "ubDom\<cdot>(receiver_o x) = {\<C> ''DoNotUse_5cf0af_o''}"
   by(simp add: receiver_o_def)
 
 lemma receiver_o_len[simp]: "ubLen (receiver_o x) = 1"
@@ -416,61 +394,60 @@ subsection \<open>stream to SB\<close>
 
 subsubsection \<open>Intern\<close>
 
-lemma receiver_stream_dr_dom[simp]: "ubDom\<cdot>(receiver_stream_dr\<cdot>x) = {\<C> ''DoNotUse_277815_dr''}"
-  by(simp add: receiver_stream_dr.rep_eq ubdom_insert DoNotUse_277815_receiver_stream_dr_h.rep_eq)
+lemma receiver_stream_dr_dom[simp]: "ubDom\<cdot>(receiver_stream_dr\<cdot>x) = {\<C> ''DoNotUse_5cf0af_dr''}"
+  by(simp add: receiver_stream_dr.rep_eq ubdom_insert DoNotUse_5cf0af_receiver_stream_dr_h.rep_eq)
 
 lemma receiver_stream_dr_len[simp]: "ubLen (receiver_stream_dr\<cdot>x) = #x"
   apply(subst uslen_ubLen_ch3)
   apply simp
   apply(simp add: receiver_stream_dr.rep_eq)
-  apply(simp add: ubGetCh_def DoNotUse_277815_receiver_stream_dr_h.rep_eq)
+  apply(simp add: ubGetCh_def DoNotUse_5cf0af_receiver_stream_dr_h.rep_eq)
   by (simp add: tsynmap_slen usclLen_stream_def)
 
-(* SWS: Gib denen einen anderen Namen, sonst duplicat *)
 lemma receiver_stream_dr_id[simp]:
-  assumes "ubDom\<cdot>ub = {\<C> ''DoNotUse_277815_dr''} "
+  assumes "ubDom\<cdot>ub = {\<C> ''DoNotUse_5cf0af_dr''} "
     shows "receiver_stream_dr\<cdot>(receiver_get_stream_dr\<cdot>ub) = ub"
   apply(simp add: receiver_stream_dr.rep_eq receiver_get_stream_dr.rep_eq)
-  apply(simp add: DoNotUse_277815_receiver_stream_dr_h_def)
-  apply(subst tsynmap_id_xx)
+  apply(simp add: DoNotUse_5cf0af_receiver_stream_dr_h_def)
+  apply(subst tsynmap_inv_id)
   using assms tsynbundle_ctype apply fastforce
   using assms ub_id_single by blast
 
-lemma receiver_stream_ar_dom[simp]: "ubDom\<cdot>(receiver_stream_ar\<cdot>x) = {\<C> ''DoNotUse_277815_ar''}"
-  by(simp add: receiver_stream_ar.rep_eq ubdom_insert DoNotUse_277815_receiver_stream_ar_h.rep_eq)
+lemma receiver_stream_ar_dom[simp]: "ubDom\<cdot>(receiver_stream_ar\<cdot>x) = {\<C> ''DoNotUse_5cf0af_ar''}"
+  by(simp add: receiver_stream_ar.rep_eq ubdom_insert DoNotUse_5cf0af_receiver_stream_ar_h.rep_eq)
 
 lemma receiver_stream_ar_len[simp]: "ubLen (receiver_stream_ar\<cdot>x) = #x"
   apply(subst uslen_ubLen_ch3)
   apply simp
   apply(simp add: receiver_stream_ar.rep_eq)
-  apply(simp add: ubGetCh_def DoNotUse_277815_receiver_stream_ar_h.rep_eq)
+  apply(simp add: ubGetCh_def DoNotUse_5cf0af_receiver_stream_ar_h.rep_eq)
   by (simp add: tsynmap_slen usclLen_stream_def)
 
 lemma receiver_stream_ar_id[simp]:
-  assumes "ubDom\<cdot>ub = {\<C> ''DoNotUse_277815_ar''} "
+  assumes "ubDom\<cdot>ub = {\<C> ''DoNotUse_5cf0af_ar''} "
     shows "receiver_stream_ar\<cdot>(receiver_get_stream_ar\<cdot>ub) = ub"
   apply(simp add: receiver_stream_ar.rep_eq receiver_get_stream_ar.rep_eq)
-  apply(simp add: DoNotUse_277815_receiver_stream_ar_h_def)
-  apply(subst tsynmap_id_xx)
+  apply(simp add: DoNotUse_5cf0af_receiver_stream_ar_h_def)
+  apply(subst tsynmap_inv_id)
   using assms tsynbundle_ctype apply fastforce
   using assms ub_id_single by blast
 
-lemma receiver_stream_o_dom[simp]: "ubDom\<cdot>(receiver_stream_o\<cdot>x) = {\<C> ''DoNotUse_277815_o''}"
-  by(simp add: receiver_stream_o.rep_eq ubdom_insert DoNotUse_277815_receiver_stream_o_h.rep_eq)
+lemma receiver_stream_o_dom[simp]: "ubDom\<cdot>(receiver_stream_o\<cdot>x) = {\<C> ''DoNotUse_5cf0af_o''}"
+  by(simp add: receiver_stream_o.rep_eq ubdom_insert DoNotUse_5cf0af_receiver_stream_o_h.rep_eq)
 
 lemma receiver_stream_o_len[simp]: "ubLen (receiver_stream_o\<cdot>x) = #x"
   apply(subst uslen_ubLen_ch3)
   apply simp
   apply(simp add: receiver_stream_o.rep_eq)
-  apply(simp add: ubGetCh_def DoNotUse_277815_receiver_stream_o_h.rep_eq)
+  apply(simp add: ubGetCh_def DoNotUse_5cf0af_receiver_stream_o_h.rep_eq)
   by (simp add: tsynmap_slen usclLen_stream_def)
 
 lemma receiver_stream_o_id[simp]:
-  assumes "ubDom\<cdot>ub = {\<C> ''DoNotUse_277815_o''} "
+  assumes "ubDom\<cdot>ub = {\<C> ''DoNotUse_5cf0af_o''} "
     shows "receiver_stream_o\<cdot>(receiver_get_stream_o\<cdot>ub) = ub"
   apply(simp add: receiver_stream_o.rep_eq receiver_get_stream_o.rep_eq)
-  apply(simp add: DoNotUse_277815_receiver_stream_o_h_def)
-  apply(subst tsynmap_id_xx)
+  apply(simp add: DoNotUse_5cf0af_receiver_stream_o_h_def)
+  apply(subst tsynmap_inv_id)
   using assms tsynbundle_ctype apply fastforce
   using assms ub_id_single by blast
 
@@ -492,7 +469,7 @@ subsection \<open>sbElem to tsyn\<close>
 
 subsubsection \<open>Intern\<close>
 
-lemma receiverelem_dr_id[simp]: "receiverElem_get_dr (receiverElem_dr x) = x"
+lemma receiverelem_get_dr_id[simp]: "receiverElem_get_dr (receiverElem_dr x) = x"
   apply(cases x)
   apply(auto simp add: receiverElem_dr.simps)
   unfolding receiverElem_get_dr_def receiverElem_raw_dr.rep_eq
@@ -500,7 +477,7 @@ lemma receiverelem_dr_id[simp]: "receiverElem_get_dr (receiverElem_dr x) = x"
   apply (meson f_inv_into_f rangeI receiverMessage.inject)
   by(simp add: sbeNull.rep_eq)
 
-lemma receiverelem_ar_id[simp]: "receiverElem_get_ar (receiverElem_ar x) = x"
+lemma receiverelem_get_ar_id[simp]: "receiverElem_get_ar (receiverElem_ar x) = x"
   apply(cases x)
   apply(auto simp add: receiverElem_ar.simps)
   unfolding receiverElem_get_ar_def receiverElem_raw_ar.rep_eq
@@ -508,7 +485,7 @@ lemma receiverelem_ar_id[simp]: "receiverElem_get_ar (receiverElem_ar x) = x"
   apply (meson f_inv_into_f rangeI receiverMessage.inject)
   by(simp add: sbeNull.rep_eq)
 
-lemma receiverelem_o_id[simp]: "receiverElem_get_o (receiverElem_o x) = x"
+lemma receiverelem_get_o_id[simp]: "receiverElem_get_o (receiverElem_o x) = x"
   apply(cases x)
   apply(auto simp add: receiverElem_o.simps)
   unfolding receiverElem_get_o_def receiverElem_raw_o.rep_eq
@@ -519,59 +496,128 @@ lemma receiverelem_o_id[simp]: "receiverElem_get_o (receiverElem_o x) = x"
 
 subsubsection \<open>In/Out\<close>
 
-lemma receiverelemin_dr_dr_id[simp]: "receiverElem_get_dr (receiverElemIn_dr port_dr) = port_dr"
+lemma receiverelem_get_dr_in_dr_id[simp]: "receiverElem_get_dr (receiverElemIn_dr port_dr) = port_dr"
   apply(simp add: receiverElemIn_dr_def receiverElem_get_dr_def)
-  by(metis receiverElem_get_dr_def receiverelem_dr_id)
+  by(metis receiverElem_get_dr_def receiverelem_get_dr_id)
 
-lemma receiverelemout_ar_o_ar_id[simp]: "receiverElem_get_ar (receiverElemOut_ar_o port_ar port_o) = port_ar"
+lemma receiverelem_get_ar_out_ar_id[simp]: "receiverElem_get_ar (receiverElemOut_ar_o port_ar port_o) = port_ar"
   apply(simp add: receiverElemOut_ar_o_def receiverElem_get_ar_def)
-  by(metis receiverElem_get_ar_def receiverelem_ar_id)
+  by(metis receiverElem_get_ar_def receiverelem_get_ar_id)
 
-lemma receiverelemout_ar_o_o_id[simp]: "receiverElem_get_o (receiverElemOut_ar_o port_ar port_o) = port_o"
+lemma receiverelem_get_o_out_o_id[simp]: "receiverElem_get_o (receiverElemOut_ar_o port_ar port_o) = port_o"
   apply(simp add: receiverElemOut_ar_o_def receiverElem_get_o_def)
-  by(metis receiverElem_get_o_def receiverelem_o_id)
+  by(metis receiverElem_get_o_def receiverelem_get_o_id)
 
 
 subsection \<open>SB to stream\<close>
 
 subsubsection \<open>Intern\<close>
 
-lemma receiver_stream_dr_id[simp]: "receiver_get_stream_dr\<cdot>(receiver_stream_dr\<cdot>x) = x"
+lemma receiver_get_stream_dr_id[simp]: "receiver_get_stream_dr\<cdot>(receiver_stream_dr\<cdot>x) = x"
   apply(simp add: receiver_get_stream_dr.rep_eq receiver_stream_dr.rep_eq)
-  apply(simp add: ubGetCh_def DoNotUse_277815_receiver_stream_dr_h.rep_eq)
+  apply(simp add: ubGetCh_def DoNotUse_5cf0af_receiver_stream_dr_h.rep_eq)
   by (simp add: inj_def)
 
-lemma receiver_stream_ar_id[simp]: "receiver_get_stream_ar\<cdot>(receiver_stream_ar\<cdot>x) = x"
+lemma receiver_get_stream_dr_eq:
+  assumes "ubDom\<cdot>ub1 = {\<C> ''DoNotUse_5cf0af_dr''}"
+      and "ubDom\<cdot>ub2 = {\<C> ''DoNotUse_5cf0af_dr''}"
+      and "receiver_get_stream_dr\<cdot>ub1 = receiver_get_stream_dr\<cdot>ub2"
+    shows "ub1 = ub2"
+  (* TODO Doesnt work for non-generic ABPComponent *)
+  (*using assms(1) assms(2) assms(3) receiver_stream_dr_id by fastforce*)
+  sorry
+
+lemma receiver_get_stream_dr_conc[simp]:
+  assumes "\<C> ''DoNotUse_5cf0af_dr'' \<in> ubDom\<cdot>ub1"
+      and "\<C> ''DoNotUse_5cf0af_dr'' \<in> ubDom\<cdot>ub2"
+    shows "receiver_get_stream_dr\<cdot>(ubConc ub1\<cdot>ub2) = (receiver_get_stream_dr\<cdot>ub1) \<bullet> (receiver_get_stream_dr\<cdot>ub2)"
+  apply(simp add: receiver_get_stream_dr.rep_eq)
+  apply (subst ubConc_usclConc_eq)
+  using assms(1) apply blast
+  using assms(2) apply blast
+  by (simp add: tsynmap_sconc usclConc_stream_def)
+
+lemma receiver_get_stream_ar_id[simp]: "receiver_get_stream_ar\<cdot>(receiver_stream_ar\<cdot>x) = x"
   apply(simp add: receiver_get_stream_ar.rep_eq receiver_stream_ar.rep_eq)
-  apply(simp add: ubGetCh_def DoNotUse_277815_receiver_stream_ar_h.rep_eq)
+  apply(simp add: ubGetCh_def DoNotUse_5cf0af_receiver_stream_ar_h.rep_eq)
   by (simp add: inj_def)
 
-lemma receiver_stream_o_id[simp]: "receiver_get_stream_o\<cdot>(receiver_stream_o\<cdot>x) = x"
+lemma receiver_get_stream_ar_eq:
+  assumes "ubDom\<cdot>ub1 = {\<C> ''DoNotUse_5cf0af_ar''}"
+      and "ubDom\<cdot>ub2 = {\<C> ''DoNotUse_5cf0af_ar''}"
+      and "receiver_get_stream_ar\<cdot>ub1 = receiver_get_stream_ar\<cdot>ub2"
+    shows "ub1 = ub2"
+  (* TODO Doesnt work for non-generic ABPComponent *)
+  (*using assms(1) assms(2) assms(3) receiver_stream_ar_id by fastforce*)
+  sorry
+
+lemma receiver_get_stream_ar_conc[simp]:
+  assumes "\<C> ''DoNotUse_5cf0af_ar'' \<in> ubDom\<cdot>ub1"
+      and "\<C> ''DoNotUse_5cf0af_ar'' \<in> ubDom\<cdot>ub2"
+    shows "receiver_get_stream_ar\<cdot>(ubConc ub1\<cdot>ub2) = (receiver_get_stream_ar\<cdot>ub1) \<bullet> (receiver_get_stream_ar\<cdot>ub2)"
+  apply(simp add: receiver_get_stream_ar.rep_eq)
+  apply (subst ubConc_usclConc_eq)
+  using assms(1) apply blast
+  using assms(2) apply blast
+  by (simp add: tsynmap_sconc usclConc_stream_def)
+
+lemma receiver_get_stream_o_id[simp]: "receiver_get_stream_o\<cdot>(receiver_stream_o\<cdot>x) = x"
   apply(simp add: receiver_get_stream_o.rep_eq receiver_stream_o.rep_eq)
-  apply(simp add: ubGetCh_def DoNotUse_277815_receiver_stream_o_h.rep_eq)
+  apply(simp add: ubGetCh_def DoNotUse_5cf0af_receiver_stream_o_h.rep_eq)
   by (simp add: inj_def)
+
+lemma receiver_get_stream_o_eq:
+  assumes "ubDom\<cdot>ub1 = {\<C> ''DoNotUse_5cf0af_o''}"
+      and "ubDom\<cdot>ub2 = {\<C> ''DoNotUse_5cf0af_o''}"
+      and "receiver_get_stream_o\<cdot>ub1 = receiver_get_stream_o\<cdot>ub2"
+    shows "ub1 = ub2"
+  (* TODO Doesnt work for non-generic ABPComponent *)
+  (*using assms(1) assms(2) assms(3) receiver_stream_o_id by fastforce*)
+  sorry
+
+lemma receiver_get_stream_o_conc[simp]:
+  assumes "\<C> ''DoNotUse_5cf0af_o'' \<in> ubDom\<cdot>ub1"
+      and "\<C> ''DoNotUse_5cf0af_o'' \<in> ubDom\<cdot>ub2"
+    shows "receiver_get_stream_o\<cdot>(ubConc ub1\<cdot>ub2) = (receiver_get_stream_o\<cdot>ub1) \<bullet> (receiver_get_stream_o\<cdot>ub2)"
+  apply(simp add: receiver_get_stream_o.rep_eq)
+  apply (subst ubConc_usclConc_eq)
+  using assms(1) apply blast
+  using assms(2) apply blast
+  by (simp add: tsynmap_sconc usclConc_stream_def)
 
 
 subsubsection \<open>In/Out\<close>
 
-lemma receiverin_stream_dr_dr_id[simp]: "receiver_get_stream_dr\<cdot>(receiverIn_stream_dr\<cdot>port_dr) = port_dr"
+lemma receiver_get_stream_dr_in_dr_id[simp]: "receiver_get_stream_dr\<cdot>(receiverIn_stream_dr\<cdot>port_dr) = port_dr"
   apply(auto simp add: receiver_get_stream_dr.rep_eq receiverIn_stream_dr_def ubclUnion_ubundle_def)
-  by (metis receiver_get_stream_dr.rep_eq receiver_stream_dr_id)
+  by (metis receiver_get_stream_dr.rep_eq receiver_get_stream_dr_id)
 
-lemma receiverout_stream_ar_o_ar_id[simp]: "receiver_get_stream_ar\<cdot>(receiverOut_stream_ar_o\<cdot>port_ar\<cdot>port_o) = port_ar"
+lemma receiver_get_stream_ar_out_ar_id[simp]: "receiver_get_stream_ar\<cdot>(receiverOut_stream_ar_o\<cdot>port_ar\<cdot>port_o) = port_ar"
   apply(auto simp add: receiver_get_stream_ar.rep_eq receiverOut_stream_ar_o_def ubclUnion_ubundle_def)
-  by (metis receiver_get_stream_ar.rep_eq receiver_stream_ar_id)
+  by (metis receiver_get_stream_ar.rep_eq receiver_get_stream_ar_id)
 
-lemma receiverout_stream_ar_o_o_id[simp]: "receiver_get_stream_o\<cdot>(receiverOut_stream_ar_o\<cdot>port_ar\<cdot>port_o) = port_o"
+lemma receiver_get_stream_o_out_o_id[simp]: "receiver_get_stream_o\<cdot>(receiverOut_stream_ar_o\<cdot>port_ar\<cdot>port_o) = port_o"
   apply(auto simp add: receiver_get_stream_o.rep_eq receiverOut_stream_ar_o_def ubclUnion_ubundle_def)
-  by (metis receiver_get_stream_o.rep_eq receiver_stream_o_id)
+  by (metis receiver_get_stream_o.rep_eq receiver_get_stream_o_id)
 
 
 subsection \<open>tsyn to SB to one-element stream\<close>
 
+subsubsection \<open>Intern\<close>
+
+lemma receiver_get_stream_dr_single[simp]: "receiver_get_stream_dr\<cdot>(receiver_dr x) = \<up>x"
+  sorry
+
+lemma receiver_get_stream_ar_single[simp]: "receiver_get_stream_ar\<cdot>(receiver_ar x) = \<up>x"
+  sorry
+
+lemma receiver_get_stream_o_single[simp]: "receiver_get_stream_o\<cdot>(receiver_o x) = \<up>x"
+  sorry
+
+
 subsubsection \<open>In/Out\<close>
 
-lemma receiverin_dr_dr_id[simp]: "receiver_get_stream_dr\<cdot>(receiverIn_dr port_dr) = \<up>port_dr"
+lemma receiver_get_stream_dr_single_in_dr_id[simp]: "receiver_get_stream_dr\<cdot>(receiverIn_dr port_dr) = \<up>port_dr"
   apply(simp add: receiver_get_stream_dr_def receiverIn_dr_def)
   apply(subst sbe2sb_getch)
   apply(auto simp add: receiverDom_def receiverElemIn_dr_def)
@@ -581,7 +627,7 @@ lemma receiverin_dr_dr_id[simp]: "receiver_get_stream_dr\<cdot>(receiverIn_dr po
   apply(simp add: inj_def)
   by(simp add: sbeNull.rep_eq)
 
-lemma receiverout_ar_o_ar_id[simp]: "receiver_get_stream_ar\<cdot>(receiverOut_ar_o port_ar port_o) = \<up>port_ar"
+lemma receiver_get_stream_ar_single_out_ar_id[simp]: "receiver_get_stream_ar\<cdot>(receiverOut_ar_o port_ar port_o) = \<up>port_ar"
   apply(simp add: receiver_get_stream_ar_def receiverOut_ar_o_def)
   apply(subst sbe2sb_getch)
   apply(auto simp add: receiverDom_def receiverElemOut_ar_o_def)
@@ -591,7 +637,7 @@ lemma receiverout_ar_o_ar_id[simp]: "receiver_get_stream_ar\<cdot>(receiverOut_a
   apply(simp add: inj_def)
   by(simp add: sbeNull.rep_eq)
 
-lemma receiverout_ar_o_o_id[simp]: "receiver_get_stream_o\<cdot>(receiverOut_ar_o port_ar port_o) = \<up>port_o"
+lemma receiver_get_stream_o_single_out_o_id[simp]: "receiver_get_stream_o\<cdot>(receiverOut_ar_o port_ar port_o) = \<up>port_o"
   apply(simp add: receiver_get_stream_o_def receiverOut_ar_o_def)
   apply(subst sbe2sb_getch)
   apply(auto simp add: receiverDom_def receiverElemOut_ar_o_def)
@@ -600,6 +646,28 @@ lemma receiverout_ar_o_o_id[simp]: "receiver_get_stream_o\<cdot>(receiverOut_ar_
   unfolding receiverElem_get_o_def receiverElem_raw_o.rep_eq
   apply(simp add: inj_def)
   by(simp add: sbeNull.rep_eq)
+
+
+section \<open>More Setter-Lemmas\<close>
+
+subsection \<open>SB to stream\<close>
+
+subsubsection \<open>Intern\<close>
+
+lemma receiver_stream_dr_conc:
+  "receiver_stream_dr\<cdot>(\<up>elem \<bullet> s) = ubConc (receiver_dr elem)\<cdot>(receiver_stream_dr\<cdot>s)"
+  apply (rule receiver_get_stream_dr_eq)
+  by simp_all
+
+lemma receiver_stream_ar_conc:
+  "receiver_stream_ar\<cdot>(\<up>elem \<bullet> s) = ubConc (receiver_ar elem)\<cdot>(receiver_stream_ar\<cdot>s)"
+  apply (rule receiver_get_stream_ar_eq)
+  by simp_all
+
+lemma receiver_stream_o_conc:
+  "receiver_stream_o\<cdot>(\<up>elem \<bullet> s) = ubConc (receiver_o elem)\<cdot>(receiver_stream_o\<cdot>s)"
+  apply (rule receiver_get_stream_o_eq)
+  by simp_all
 
 
 section \<open>Step-wise lemmata for the transition function\<close>
