abp/SenderAutomaton.thy
@@ -3,35 +3,13 @@
  * This file was generated from Sender.maa and will be overridden when changed. To change
  * permanently, consider changing the model itself.
  *
- * isartransformer 1.0.0
+ * Generated on Oct 3, 2018 9:18:08 PM by isartransformer 1.0.0
  *)
 theory SenderAutomaton
   imports bundle.tsynBundle automat.dAutomaton
 
 begin
 
-
-(* TODO Move to tsynStream and find a name for it, the proposed "tsynmap_id" already exists *)
-lemma tsynmap_id_xx[simp]: "tsynDom\<cdot>tsyn \<subseteq> range F \<Longrightarrow> tsynMap F\<cdot>(tsynMap (inv F)\<cdot>tsyn) = tsyn"
-  apply(induction tsyn rule: ind)
-    apply simp_all
-  apply(rename_tac x xs)
-  apply(case_tac x)
-   apply(auto simp add: tsynmap_sconc_msg tsynmap_sconc_null)
-  by(auto simp add: tsyndom_sconc_msg tsyndom_sconc_null f_inv_into_f)
-
-(* TODO: Move to tsynBundle *)
-lemma tsynbundle_ctype: fixes ub::"'m::message tsyn SB"
-  shows "c\<in>ubDom\<cdot>ub \<Longrightarrow> tsynDom\<cdot>(ub . c) \<subseteq> (ctype c)"
-  apply(simp add: tsyndom_insert)
-  using usclOkay_stream_def ctype_tsyn_def
-  by (smt ctype_tsyn_iff mem_Collect_eq subsetCE subsetI ubdom_channel_usokay ubgetch_insert)
-
-(* TODO: Move to UBundle *)
-lemma ub_id_single: "ubDom\<cdot>ub = {c} \<Longrightarrow> Abs_ubundle [c \<mapsto> ub  .  c] = ub"
-  apply(rule ub_eq)
-  apply simp
-  by (simp add: ubWell_single_channel ubdom_ubrep_eq ubgetch_insert)+
 
 (* Helper for easier generation *)
 fun prepend :: "'a::type list \<Rightarrow> 'a \<Rightarrow> 'a list" where
@@ -42,7 +20,7 @@ section \<open>Datatype\<close>
 
 subsection \<open>Definition\<close>
 
-datatype ('e::countable) senderMessage = DoNotUse_e8177d_SenderBool "bool" | DoNotUse_e8177d_SenderE "'e" | DoNotUse_e8177d_SenderPair_E_Bool "('e\<times>bool)"
+datatype ('e::countable) senderMessage = DoNotUse_8f2b50_SenderBool "bool" | DoNotUse_8f2b50_SenderE "'e" | DoNotUse_8f2b50_SenderPair_E_Bool "('e\<times>bool)"
 
 instance senderMessage :: (countable) countable
   apply(intro_classes)
@@ -52,9 +30,9 @@ instantiation senderMessage :: (countable) message
 begin
   fun ctype_senderMessage :: "channel \<Rightarrow> ('e::countable) senderMessage set" where
   "ctype_senderMessage c = (
-    if c = \<C> ''DoNotUse_e8177d_as'' then range DoNotUse_e8177d_SenderBool else
-    if c = \<C> ''DoNotUse_e8177d_i'' then range DoNotUse_e8177d_SenderE else
-    if c = \<C> ''DoNotUse_e8177d_ds'' then range DoNotUse_e8177d_SenderPair_E_Bool else
+    if c = \<C> ''DoNotUse_8f2b50_as'' then range DoNotUse_8f2b50_SenderBool else
+    if c = \<C> ''DoNotUse_8f2b50_i'' then range DoNotUse_8f2b50_SenderE else
+    if c = \<C> ''DoNotUse_8f2b50_ds'' then range DoNotUse_8f2b50_SenderPair_E_Bool else
     undefined)"
   instance
     by(intro_classes)
@@ -64,10 +42,10 @@ end
 subsection \<open>Domain and Range\<close>
 
 definition senderDom :: "channel set" where
-"senderDom = {\<C> ''DoNotUse_e8177d_as'', \<C> ''DoNotUse_e8177d_i''}"
+"senderDom = {\<C> ''DoNotUse_8f2b50_as'', \<C> ''DoNotUse_8f2b50_i''}"
 
 definition senderRan :: "channel set" where
-"senderRan = {\<C> ''DoNotUse_e8177d_ds''}"
+"senderRan = {\<C> ''DoNotUse_8f2b50_ds''}"
 
 
 section \<open>Setter\<close>
@@ -76,19 +54,19 @@ subsection \<open>type to sbElem\<close>
 
 (* Do not use this, use senderElemIn_as_i instead *)
 lift_definition senderElem_raw_as :: "bool \<Rightarrow> ('e::countable) senderMessage tsyn sbElem" is
-"\<lambda>x. [\<C> ''DoNotUse_e8177d_as'' \<mapsto> Msg (DoNotUse_e8177d_SenderBool x)]"
+"\<lambda>x. [\<C> ''DoNotUse_8f2b50_as'' \<mapsto> Msg (DoNotUse_8f2b50_SenderBool x)]"
   unfolding sbElemWell_def usclOkay_stream_def ctype_tsyn_def
   by simp
 
 (* Do not use this, use senderElemIn_as_i instead *)
 lift_definition senderElem_raw_i :: "'e \<Rightarrow> ('e::countable) senderMessage tsyn sbElem" is
-"\<lambda>x. [\<C> ''DoNotUse_e8177d_i'' \<mapsto> Msg (DoNotUse_e8177d_SenderE x)]"
+"\<lambda>x. [\<C> ''DoNotUse_8f2b50_i'' \<mapsto> Msg (DoNotUse_8f2b50_SenderE x)]"
   unfolding sbElemWell_def usclOkay_stream_def ctype_tsyn_def
   by simp
 
 (* Do not use this, use senderElemOut_ds instead *)
 lift_definition senderElem_raw_ds :: "('e\<times>bool) \<Rightarrow> ('e::countable) senderMessage tsyn sbElem" is
-"\<lambda>x. [\<C> ''DoNotUse_e8177d_ds'' \<mapsto> Msg (DoNotUse_e8177d_SenderPair_E_Bool x)]"
+"\<lambda>x. [\<C> ''DoNotUse_8f2b50_ds'' \<mapsto> Msg (DoNotUse_8f2b50_SenderPair_E_Bool x)]"
   unfolding sbElemWell_def usclOkay_stream_def ctype_tsyn_def
   by simp
 
@@ -100,17 +78,17 @@ subsubsection \<open>Intern\<close>
 (* Do not use this, use senderElemIn_as_i instead *)
 fun senderElem_as :: "bool tsyn \<Rightarrow> ('e::countable) senderMessage tsyn sbElem" where
 "senderElem_as (Msg port_as) = senderElem_raw_as port_as" |
-"senderElem_as null = sbeNull {\<C> ''DoNotUse_e8177d_as''}"
+"senderElem_as null = sbeNull {\<C> ''DoNotUse_8f2b50_as''}"
 
 (* Do not use this, use senderElemIn_as_i instead *)
 fun senderElem_i :: "'e tsyn \<Rightarrow> ('e::countable) senderMessage tsyn sbElem" where
 "senderElem_i (Msg port_i) = senderElem_raw_i port_i" |
-"senderElem_i null = sbeNull {\<C> ''DoNotUse_e8177d_i''}"
+"senderElem_i null = sbeNull {\<C> ''DoNotUse_8f2b50_i''}"
 
 (* Do not use this, use senderElemOut_ds instead *)
 fun senderElem_ds :: "('e\<times>bool) tsyn \<Rightarrow> ('e::countable) senderMessage tsyn sbElem" where
 "senderElem_ds (Msg port_ds) = senderElem_raw_ds port_ds" |
-"senderElem_ds null = sbeNull {\<C> ''DoNotUse_e8177d_ds''}"
+"senderElem_ds null = sbeNull {\<C> ''DoNotUse_8f2b50_ds''}"
 
 declare senderElem_as.simps[simp del]
 
@@ -157,21 +135,21 @@ subsubsection \<open>Intern\<close>
 (* Do not use this, use senderIn_list_as_i instead *)
 fun sender_list_as :: "(bool tsyn) list \<Rightarrow> ('e::countable) senderMessage tsyn SB" where
 "sender_list_as (x#xs) = ubConcEq (sender_as x)\<cdot>(sender_list_as xs)" |
-"sender_list_as []     = ubLeast {\<C> ''DoNotUse_e8177d_as''}"
+"sender_list_as []     = ubLeast {\<C> ''DoNotUse_8f2b50_as''}"
 
 declare sender_list_as.simps[simp del]
 
 (* Do not use this, use senderIn_list_as_i instead *)
 fun sender_list_i :: "('e tsyn) list \<Rightarrow> ('e::countable) senderMessage tsyn SB" where
 "sender_list_i (x#xs) = ubConcEq (sender_i x)\<cdot>(sender_list_i xs)" |
-"sender_list_i []     = ubLeast {\<C> ''DoNotUse_e8177d_i''}"
+"sender_list_i []     = ubLeast {\<C> ''DoNotUse_8f2b50_i''}"
 
 declare sender_list_i.simps[simp del]
 
 (* Do not use this, use senderOut_list_ds instead *)
 fun sender_list_ds :: "(('e\<times>bool) tsyn) list \<Rightarrow> ('e::countable) senderMessage tsyn SB" where
 "sender_list_ds (x#xs) = ubConcEq (sender_ds x)\<cdot>(sender_list_ds xs)" |
-"sender_list_ds []     = ubLeast {\<C> ''DoNotUse_e8177d_ds''}"
+"sender_list_ds []     = ubLeast {\<C> ''DoNotUse_8f2b50_ds''}"
 
 declare sender_list_ds.simps[simp del]
 
@@ -193,44 +171,44 @@ subsection \<open>stream to SB\<close>
 
 subsubsection \<open>Intern\<close>
 
-lift_definition DoNotUse_e8177d_sender_stream_as_h :: "bool tsyn stream \<Rightarrow> ('e::countable) senderMessage tsyn SB" is
-"\<lambda> s. [(\<C> ''DoNotUse_e8177d_as'') \<mapsto> (tsynMap (DoNotUse_e8177d_SenderBool)\<cdot>s)]"
+lift_definition DoNotUse_8f2b50_sender_stream_as_h :: "bool tsyn stream \<Rightarrow> ('e::countable) senderMessage tsyn SB" is
+"\<lambda> s. [(\<C> ''DoNotUse_8f2b50_as'') \<mapsto> (tsynMap (DoNotUse_8f2b50_SenderBool)\<cdot>s)]"
   unfolding ubWell_def usclOkay_stream_def ctype_tsyn_def
   by auto
 
 (* Do not use this, use senderIn_stream_as_i instead *)
 lift_definition sender_stream_as :: "(bool) tsyn stream \<rightarrow> ('e::countable) senderMessage tsyn SB" is
-"DoNotUse_e8177d_sender_stream_as_h"
-  apply(auto simp add: cfun_def DoNotUse_e8177d_sender_stream_as_h_def map_fun_def comp_def)
+"DoNotUse_8f2b50_sender_stream_as_h"
+  apply(auto simp add: cfun_def DoNotUse_8f2b50_sender_stream_as_h_def map_fun_def comp_def)
   apply(rule cont_Abs_UB)
   apply(simp add: option_one_cont)
-  by (metis DoNotUse_e8177d_sender_stream_as_h.rep_eq ubrep_well)
+  by (metis DoNotUse_8f2b50_sender_stream_as_h.rep_eq ubrep_well)
 
-lift_definition DoNotUse_e8177d_sender_stream_i_h :: "'e tsyn stream \<Rightarrow> ('e::countable) senderMessage tsyn SB" is
-"\<lambda> s. [(\<C> ''DoNotUse_e8177d_i'') \<mapsto> (tsynMap (DoNotUse_e8177d_SenderE)\<cdot>s)]"
+lift_definition DoNotUse_8f2b50_sender_stream_i_h :: "'e tsyn stream \<Rightarrow> ('e::countable) senderMessage tsyn SB" is
+"\<lambda> s. [(\<C> ''DoNotUse_8f2b50_i'') \<mapsto> (tsynMap (DoNotUse_8f2b50_SenderE)\<cdot>s)]"
   unfolding ubWell_def usclOkay_stream_def ctype_tsyn_def
   by auto
 
 (* Do not use this, use senderIn_stream_as_i instead *)
 lift_definition sender_stream_i :: "('e) tsyn stream \<rightarrow> ('e::countable) senderMessage tsyn SB" is
-"DoNotUse_e8177d_sender_stream_i_h"
-  apply(auto simp add: cfun_def DoNotUse_e8177d_sender_stream_i_h_def map_fun_def comp_def)
+"DoNotUse_8f2b50_sender_stream_i_h"
+  apply(auto simp add: cfun_def DoNotUse_8f2b50_sender_stream_i_h_def map_fun_def comp_def)
   apply(rule cont_Abs_UB)
   apply(simp add: option_one_cont)
-  by (metis DoNotUse_e8177d_sender_stream_i_h.rep_eq ubrep_well)
+  by (metis DoNotUse_8f2b50_sender_stream_i_h.rep_eq ubrep_well)
 
-lift_definition DoNotUse_e8177d_sender_stream_ds_h :: "('e\<times>bool) tsyn stream \<Rightarrow> ('e::countable) senderMessage tsyn SB" is
-"\<lambda> s. [(\<C> ''DoNotUse_e8177d_ds'') \<mapsto> (tsynMap (DoNotUse_e8177d_SenderPair_E_Bool)\<cdot>s)]"
+lift_definition DoNotUse_8f2b50_sender_stream_ds_h :: "('e\<times>bool) tsyn stream \<Rightarrow> ('e::countable) senderMessage tsyn SB" is
+"\<lambda> s. [(\<C> ''DoNotUse_8f2b50_ds'') \<mapsto> (tsynMap (DoNotUse_8f2b50_SenderPair_E_Bool)\<cdot>s)]"
   unfolding ubWell_def usclOkay_stream_def ctype_tsyn_def
   by auto
 
 (* Do not use this, use senderOut_stream_ds instead *)
 lift_definition sender_stream_ds :: "(('e\<times>bool)) tsyn stream \<rightarrow> ('e::countable) senderMessage tsyn SB" is
-"DoNotUse_e8177d_sender_stream_ds_h"
-  apply(auto simp add: cfun_def DoNotUse_e8177d_sender_stream_ds_h_def map_fun_def comp_def)
+"DoNotUse_8f2b50_sender_stream_ds_h"
+  apply(auto simp add: cfun_def DoNotUse_8f2b50_sender_stream_ds_h_def map_fun_def comp_def)
   apply(rule cont_Abs_UB)
   apply(simp add: option_one_cont)
-  by (metis DoNotUse_e8177d_sender_stream_ds_h.rep_eq ubrep_well)
+  by (metis DoNotUse_8f2b50_sender_stream_ds_h.rep_eq ubrep_well)
 
 
 subsubsection \<open>In/Out\<close>
@@ -248,27 +226,27 @@ section \<open>Getter\<close>
 subsection \<open>sbElem to tsyn\<close>
 
 definition senderElem_get_as :: "('e::countable) senderMessage tsyn sbElem \<Rightarrow> (bool) tsyn" where
-"senderElem_get_as sbe = tsynApplyElem (inv DoNotUse_e8177d_SenderBool) ((Rep_sbElem sbe) \<rightharpoonup> (\<C> ''DoNotUse_e8177d_as''))"
+"senderElem_get_as sbe = tsynApplyElem (inv DoNotUse_8f2b50_SenderBool) ((Rep_sbElem sbe) \<rightharpoonup> (\<C> ''DoNotUse_8f2b50_as''))"
 
 definition senderElem_get_i :: "('e::countable) senderMessage tsyn sbElem \<Rightarrow> ('e) tsyn" where
-"senderElem_get_i sbe = tsynApplyElem (inv DoNotUse_e8177d_SenderE) ((Rep_sbElem sbe) \<rightharpoonup> (\<C> ''DoNotUse_e8177d_i''))"
+"senderElem_get_i sbe = tsynApplyElem (inv DoNotUse_8f2b50_SenderE) ((Rep_sbElem sbe) \<rightharpoonup> (\<C> ''DoNotUse_8f2b50_i''))"
 
 definition senderElem_get_ds :: "('e::countable) senderMessage tsyn sbElem \<Rightarrow> (('e\<times>bool)) tsyn" where
-"senderElem_get_ds sbe = tsynApplyElem (inv DoNotUse_e8177d_SenderPair_E_Bool) ((Rep_sbElem sbe) \<rightharpoonup> (\<C> ''DoNotUse_e8177d_ds''))"
+"senderElem_get_ds sbe = tsynApplyElem (inv DoNotUse_8f2b50_SenderPair_E_Bool) ((Rep_sbElem sbe) \<rightharpoonup> (\<C> ''DoNotUse_8f2b50_ds''))"
 
 
 subsection \<open>SB to stream\<close>
 
 lift_definition sender_get_stream_as :: "('e::countable) senderMessage tsyn SB \<rightarrow> bool tsyn stream" is
-"\<lambda>sb. tsynMap (inv DoNotUse_e8177d_SenderBool)\<cdot>(sb . (\<C> ''DoNotUse_e8177d_as''))"
+"\<lambda>sb. tsynMap (inv DoNotUse_8f2b50_SenderBool)\<cdot>(sb . (\<C> ''DoNotUse_8f2b50_as''))"
   by(simp add: cfun_def)
 
 lift_definition sender_get_stream_i :: "('e::countable) senderMessage tsyn SB \<rightarrow> 'e tsyn stream" is
-"\<lambda>sb. tsynMap (inv DoNotUse_e8177d_SenderE)\<cdot>(sb . (\<C> ''DoNotUse_e8177d_i''))"
+"\<lambda>sb. tsynMap (inv DoNotUse_8f2b50_SenderE)\<cdot>(sb . (\<C> ''DoNotUse_8f2b50_i''))"
   by(simp add: cfun_def)
 
 lift_definition sender_get_stream_ds :: "('e::countable) senderMessage tsyn SB \<rightarrow> ('e\<times>bool) tsyn stream" is
-"\<lambda>sb. tsynMap (inv DoNotUse_e8177d_SenderPair_E_Bool)\<cdot>(sb . (\<C> ''DoNotUse_e8177d_ds''))"
+"\<lambda>sb. tsynMap (inv DoNotUse_8f2b50_SenderPair_E_Bool)\<cdot>(sb . (\<C> ''DoNotUse_8f2b50_ds''))"
   by(simp add: cfun_def)
 
 
@@ -404,34 +382,34 @@ subsection \<open>tsyn to sbElem/SB\<close>
 
 subsubsection \<open>Intern\<close>
 
-lemma senderelem_as_dom[simp]: "sbeDom (senderElem_as x) = {\<C> ''DoNotUse_e8177d_as''}"
+lemma senderelem_as_dom[simp]: "sbeDom (senderElem_as x) = {\<C> ''DoNotUse_8f2b50_as''}"
   apply(cases x)
   apply(simp add: senderElem_as.simps sbeDom_def senderElem_raw_as.rep_eq)
   by(simp add: senderElem_as.simps)
 
-lemma senderelem_i_dom[simp]: "sbeDom (senderElem_i x) = {\<C> ''DoNotUse_e8177d_i''}"
+lemma senderelem_i_dom[simp]: "sbeDom (senderElem_i x) = {\<C> ''DoNotUse_8f2b50_i''}"
   apply(cases x)
   apply(simp add: senderElem_i.simps sbeDom_def senderElem_raw_i.rep_eq)
   by(simp add: senderElem_i.simps)
 
-lemma senderelem_ds_dom[simp]: "sbeDom (senderElem_ds x) = {\<C> ''DoNotUse_e8177d_ds''}"
+lemma senderelem_ds_dom[simp]: "sbeDom (senderElem_ds x) = {\<C> ''DoNotUse_8f2b50_ds''}"
   apply(cases x)
   apply(simp add: senderElem_ds.simps sbeDom_def senderElem_raw_ds.rep_eq)
   by(simp add: senderElem_ds.simps)
 
-lemma sender_as_dom[simp]: "ubDom\<cdot>(sender_as x) = {\<C> ''DoNotUse_e8177d_as''}"
+lemma sender_as_dom[simp]: "ubDom\<cdot>(sender_as x) = {\<C> ''DoNotUse_8f2b50_as''}"
   by(simp add: sender_as_def)
 
 lemma sender_as_len[simp]: "ubLen (sender_as x) = 1"
   by(simp add: sender_as_def)
 
-lemma sender_i_dom[simp]: "ubDom\<cdot>(sender_i x) = {\<C> ''DoNotUse_e8177d_i''}"
+lemma sender_i_dom[simp]: "ubDom\<cdot>(sender_i x) = {\<C> ''DoNotUse_8f2b50_i''}"
   by(simp add: sender_i_def)
 
 lemma sender_i_len[simp]: "ubLen (sender_i x) = 1"
   by(simp add: sender_i_def)
 
-lemma sender_ds_dom[simp]: "ubDom\<cdot>(sender_ds x) = {\<C> ''DoNotUse_e8177d_ds''}"
+lemma sender_ds_dom[simp]: "ubDom\<cdot>(sender_ds x) = {\<C> ''DoNotUse_8f2b50_ds''}"
   by(simp add: sender_ds_def)
 
 lemma sender_ds_len[simp]: "ubLen (sender_ds x) = 1"
@@ -463,60 +441,60 @@ subsection \<open>stream to SB\<close>
 
 subsubsection \<open>Intern\<close>
 
-lemma sender_stream_as_dom[simp]: "ubDom\<cdot>(sender_stream_as\<cdot>x) = {\<C> ''DoNotUse_e8177d_as''}"
-  by(simp add: sender_stream_as.rep_eq ubdom_insert DoNotUse_e8177d_sender_stream_as_h.rep_eq)
+lemma sender_stream_as_dom[simp]: "ubDom\<cdot>(sender_stream_as\<cdot>x) = {\<C> ''DoNotUse_8f2b50_as''}"
+  by(simp add: sender_stream_as.rep_eq ubdom_insert DoNotUse_8f2b50_sender_stream_as_h.rep_eq)
 
 lemma sender_stream_as_len[simp]: "ubLen (sender_stream_as\<cdot>x) = #x"
   apply(subst uslen_ubLen_ch3)
   apply simp
   apply(simp add: sender_stream_as.rep_eq)
-  apply(simp add: ubGetCh_def DoNotUse_e8177d_sender_stream_as_h.rep_eq)
+  apply(simp add: ubGetCh_def DoNotUse_8f2b50_sender_stream_as_h.rep_eq)
   by (simp add: tsynmap_slen usclLen_stream_def)
 
 lemma sender_stream_as_id[simp]:
-  assumes "ubDom\<cdot>ub = {\<C> ''DoNotUse_e8177d_as''} "
+  assumes "ubDom\<cdot>ub = {\<C> ''DoNotUse_8f2b50_as''} "
     shows "sender_stream_as\<cdot>(sender_get_stream_as\<cdot>ub) = ub"
   apply(simp add: sender_stream_as.rep_eq sender_get_stream_as.rep_eq)
-  apply(simp add: DoNotUse_e8177d_sender_stream_as_h_def)
-  apply(subst tsynmap_id_xx)
+  apply(simp add: DoNotUse_8f2b50_sender_stream_as_h_def)
+  apply(subst tsynmap_inv_id)
   using assms tsynbundle_ctype apply fastforce
   using assms ub_id_single by blast
 
-lemma sender_stream_i_dom[simp]: "ubDom\<cdot>(sender_stream_i\<cdot>x) = {\<C> ''DoNotUse_e8177d_i''}"
-  by(simp add: sender_stream_i.rep_eq ubdom_insert DoNotUse_e8177d_sender_stream_i_h.rep_eq)
+lemma sender_stream_i_dom[simp]: "ubDom\<cdot>(sender_stream_i\<cdot>x) = {\<C> ''DoNotUse_8f2b50_i''}"
+  by(simp add: sender_stream_i.rep_eq ubdom_insert DoNotUse_8f2b50_sender_stream_i_h.rep_eq)
 
 lemma sender_stream_i_len[simp]: "ubLen (sender_stream_i\<cdot>x) = #x"
   apply(subst uslen_ubLen_ch3)
   apply simp
   apply(simp add: sender_stream_i.rep_eq)
-  apply(simp add: ubGetCh_def DoNotUse_e8177d_sender_stream_i_h.rep_eq)
+  apply(simp add: ubGetCh_def DoNotUse_8f2b50_sender_stream_i_h.rep_eq)
   by (simp add: tsynmap_slen usclLen_stream_def)
 
 lemma sender_stream_i_id[simp]:
-  assumes "ubDom\<cdot>ub = {\<C> ''DoNotUse_e8177d_i''} "
+  assumes "ubDom\<cdot>ub = {\<C> ''DoNotUse_8f2b50_i''} "
     shows "sender_stream_i\<cdot>(sender_get_stream_i\<cdot>ub) = ub"
   apply(simp add: sender_stream_i.rep_eq sender_get_stream_i.rep_eq)
-  apply(simp add: DoNotUse_e8177d_sender_stream_i_h_def)
-  apply(subst tsynmap_id_xx)
+  apply(simp add: DoNotUse_8f2b50_sender_stream_i_h_def)
+  apply(subst tsynmap_inv_id)
   using assms tsynbundle_ctype apply fastforce
   using assms ub_id_single by blast
 
-lemma sender_stream_ds_dom[simp]: "ubDom\<cdot>(sender_stream_ds\<cdot>x) = {\<C> ''DoNotUse_e8177d_ds''}"
-  by(simp add: sender_stream_ds.rep_eq ubdom_insert DoNotUse_e8177d_sender_stream_ds_h.rep_eq)
+lemma sender_stream_ds_dom[simp]: "ubDom\<cdot>(sender_stream_ds\<cdot>x) = {\<C> ''DoNotUse_8f2b50_ds''}"
+  by(simp add: sender_stream_ds.rep_eq ubdom_insert DoNotUse_8f2b50_sender_stream_ds_h.rep_eq)
 
 lemma sender_stream_ds_len[simp]: "ubLen (sender_stream_ds\<cdot>x) = #x"
   apply(subst uslen_ubLen_ch3)
   apply simp
   apply(simp add: sender_stream_ds.rep_eq)
-  apply(simp add: ubGetCh_def DoNotUse_e8177d_sender_stream_ds_h.rep_eq)
+  apply(simp add: ubGetCh_def DoNotUse_8f2b50_sender_stream_ds_h.rep_eq)
   by (simp add: tsynmap_slen usclLen_stream_def)
 
 lemma sender_stream_ds_id[simp]:
-  assumes "ubDom\<cdot>ub = {\<C> ''DoNotUse_e8177d_ds''} "
+  assumes "ubDom\<cdot>ub = {\<C> ''DoNotUse_8f2b50_ds''} "
     shows "sender_stream_ds\<cdot>(sender_get_stream_ds\<cdot>ub) = ub"
   apply(simp add: sender_stream_ds.rep_eq sender_get_stream_ds.rep_eq)
-  apply(simp add: DoNotUse_e8177d_sender_stream_ds_h_def)
-  apply(subst tsynmap_id_xx)
+  apply(simp add: DoNotUse_8f2b50_sender_stream_ds_h_def)
+  apply(subst tsynmap_inv_id)
   using assms tsynbundle_ctype apply fastforce
   using assms ub_id_single by blast
 
@@ -538,7 +516,7 @@ subsection \<open>sbElem to tsyn\<close>
 
 subsubsection \<open>Intern\<close>
 
-lemma senderelem_as_id[simp]: "senderElem_get_as (senderElem_as x) = x"
+lemma senderelem_get_as_id[simp]: "senderElem_get_as (senderElem_as x) = x"
   apply(cases x)
   apply(auto simp add: senderElem_as.simps)
   unfolding senderElem_get_as_def senderElem_raw_as.rep_eq
@@ -546,7 +524,7 @@ lemma senderelem_as_id[simp]: "senderElem_get_as (senderElem_as x) = x"
   apply (meson f_inv_into_f rangeI senderMessage.inject)
   by(simp add: sbeNull.rep_eq)
 
-lemma senderelem_i_id[simp]: "senderElem_get_i (senderElem_i x) = x"
+lemma senderelem_get_i_id[simp]: "senderElem_get_i (senderElem_i x) = x"
   apply(cases x)
   apply(auto simp add: senderElem_i.simps)
   unfolding senderElem_get_i_def senderElem_raw_i.rep_eq
@@ -554,7 +532,7 @@ lemma senderelem_i_id[simp]: "senderElem_get_i (senderElem_i x) = x"
   apply (meson f_inv_into_f rangeI senderMessage.inject)
   by(simp add: sbeNull.rep_eq)
 
-lemma senderelem_ds_id[simp]: "senderElem_get_ds (senderElem_ds x) = x"
+lemma senderelem_get_ds_id[simp]: "senderElem_get_ds (senderElem_ds x) = x"
   apply(cases x)
   apply(auto simp add: senderElem_ds.simps)
   unfolding senderElem_get_ds_def senderElem_raw_ds.rep_eq
@@ -565,59 +543,128 @@ lemma senderelem_ds_id[simp]: "senderElem_get_ds (senderElem_ds x) = x"
 
 subsubsection \<open>In/Out\<close>
 
-lemma senderelemin_as_i_as_id[simp]: "senderElem_get_as (senderElemIn_as_i port_as port_i) = port_as"
+lemma senderelem_get_as_in_as_id[simp]: "senderElem_get_as (senderElemIn_as_i port_as port_i) = port_as"
   apply(simp add: senderElemIn_as_i_def senderElem_get_as_def)
-  by(metis senderElem_get_as_def senderelem_as_id)
+  by(metis senderElem_get_as_def senderelem_get_as_id)
 
-lemma senderelemin_as_i_i_id[simp]: "senderElem_get_i (senderElemIn_as_i port_as port_i) = port_i"
+lemma senderelem_get_i_in_i_id[simp]: "senderElem_get_i (senderElemIn_as_i port_as port_i) = port_i"
   apply(simp add: senderElemIn_as_i_def senderElem_get_i_def)
-  by(metis senderElem_get_i_def senderelem_i_id)
+  by(metis senderElem_get_i_def senderelem_get_i_id)
 
-lemma senderelemout_ds_ds_id[simp]: "senderElem_get_ds (senderElemOut_ds port_ds) = port_ds"
+lemma senderelem_get_ds_out_ds_id[simp]: "senderElem_get_ds (senderElemOut_ds port_ds) = port_ds"
   apply(simp add: senderElemOut_ds_def senderElem_get_ds_def)
-  by(metis senderElem_get_ds_def senderelem_ds_id)
+  by(metis senderElem_get_ds_def senderelem_get_ds_id)
 
 
 subsection \<open>SB to stream\<close>
 
 subsubsection \<open>Intern\<close>
 
-lemma sender_stream_as_id[simp]: "sender_get_stream_as\<cdot>(sender_stream_as\<cdot>x) = x"
+lemma sender_get_stream_as_id[simp]: "sender_get_stream_as\<cdot>(sender_stream_as\<cdot>x) = x"
   apply(simp add: sender_get_stream_as.rep_eq sender_stream_as.rep_eq)
-  apply(simp add: ubGetCh_def DoNotUse_e8177d_sender_stream_as_h.rep_eq)
+  apply(simp add: ubGetCh_def DoNotUse_8f2b50_sender_stream_as_h.rep_eq)
   by (simp add: inj_def)
 
-lemma sender_stream_i_id[simp]: "sender_get_stream_i\<cdot>(sender_stream_i\<cdot>x) = x"
+lemma sender_get_stream_as_eq:
+  assumes "ubDom\<cdot>ub1 = {\<C> ''DoNotUse_8f2b50_as''}"
+      and "ubDom\<cdot>ub2 = {\<C> ''DoNotUse_8f2b50_as''}"
+      and "sender_get_stream_as\<cdot>ub1 = sender_get_stream_as\<cdot>ub2"
+    shows "ub1 = ub2"
+  (* TODO Doesnt work for non-generic ABPComponent *)
+  (*using assms(1) assms(2) assms(3) sender_stream_as_id by fastforce*)
+  sorry
+
+lemma sender_get_stream_as_conc[simp]:
+  assumes "\<C> ''DoNotUse_8f2b50_as'' \<in> ubDom\<cdot>ub1"
+      and "\<C> ''DoNotUse_8f2b50_as'' \<in> ubDom\<cdot>ub2"
+    shows "sender_get_stream_as\<cdot>(ubConc ub1\<cdot>ub2) = (sender_get_stream_as\<cdot>ub1) \<bullet> (sender_get_stream_as\<cdot>ub2)"
+  apply(simp add: sender_get_stream_as.rep_eq)
+  apply (subst ubConc_usclConc_eq)
+  using assms(1) apply blast
+  using assms(2) apply blast
+  by (simp add: tsynmap_sconc usclConc_stream_def)
+
+lemma sender_get_stream_i_id[simp]: "sender_get_stream_i\<cdot>(sender_stream_i\<cdot>x) = x"
   apply(simp add: sender_get_stream_i.rep_eq sender_stream_i.rep_eq)
-  apply(simp add: ubGetCh_def DoNotUse_e8177d_sender_stream_i_h.rep_eq)
+  apply(simp add: ubGetCh_def DoNotUse_8f2b50_sender_stream_i_h.rep_eq)
   by (simp add: inj_def)
 
-lemma sender_stream_ds_id[simp]: "sender_get_stream_ds\<cdot>(sender_stream_ds\<cdot>x) = x"
+lemma sender_get_stream_i_eq:
+  assumes "ubDom\<cdot>ub1 = {\<C> ''DoNotUse_8f2b50_i''}"
+      and "ubDom\<cdot>ub2 = {\<C> ''DoNotUse_8f2b50_i''}"
+      and "sender_get_stream_i\<cdot>ub1 = sender_get_stream_i\<cdot>ub2"
+    shows "ub1 = ub2"
+  (* TODO Doesnt work for non-generic ABPComponent *)
+  (*using assms(1) assms(2) assms(3) sender_stream_i_id by fastforce*)
+  sorry
+
+lemma sender_get_stream_i_conc[simp]:
+  assumes "\<C> ''DoNotUse_8f2b50_i'' \<in> ubDom\<cdot>ub1"
+      and "\<C> ''DoNotUse_8f2b50_i'' \<in> ubDom\<cdot>ub2"
+    shows "sender_get_stream_i\<cdot>(ubConc ub1\<cdot>ub2) = (sender_get_stream_i\<cdot>ub1) \<bullet> (sender_get_stream_i\<cdot>ub2)"
+  apply(simp add: sender_get_stream_i.rep_eq)
+  apply (subst ubConc_usclConc_eq)
+  using assms(1) apply blast
+  using assms(2) apply blast
+  by (simp add: tsynmap_sconc usclConc_stream_def)
+
+lemma sender_get_stream_ds_id[simp]: "sender_get_stream_ds\<cdot>(sender_stream_ds\<cdot>x) = x"
   apply(simp add: sender_get_stream_ds.rep_eq sender_stream_ds.rep_eq)
-  apply(simp add: ubGetCh_def DoNotUse_e8177d_sender_stream_ds_h.rep_eq)
+  apply(simp add: ubGetCh_def DoNotUse_8f2b50_sender_stream_ds_h.rep_eq)
   by (simp add: inj_def)
+
+lemma sender_get_stream_ds_eq:
+  assumes "ubDom\<cdot>ub1 = {\<C> ''DoNotUse_8f2b50_ds''}"
+      and "ubDom\<cdot>ub2 = {\<C> ''DoNotUse_8f2b50_ds''}"
+      and "sender_get_stream_ds\<cdot>ub1 = sender_get_stream_ds\<cdot>ub2"
+    shows "ub1 = ub2"
+  (* TODO Doesnt work for non-generic ABPComponent *)
+  (*using assms(1) assms(2) assms(3) sender_stream_ds_id by fastforce*)
+  sorry
+
+lemma sender_get_stream_ds_conc[simp]:
+  assumes "\<C> ''DoNotUse_8f2b50_ds'' \<in> ubDom\<cdot>ub1"
+      and "\<C> ''DoNotUse_8f2b50_ds'' \<in> ubDom\<cdot>ub2"
+    shows "sender_get_stream_ds\<cdot>(ubConc ub1\<cdot>ub2) = (sender_get_stream_ds\<cdot>ub1) \<bullet> (sender_get_stream_ds\<cdot>ub2)"
+  apply(simp add: sender_get_stream_ds.rep_eq)
+  apply (subst ubConc_usclConc_eq)
+  using assms(1) apply blast
+  using assms(2) apply blast
+  by (simp add: tsynmap_sconc usclConc_stream_def)
 
 
 subsubsection \<open>In/Out\<close>
 
-lemma senderin_stream_as_i_as_id[simp]: "sender_get_stream_as\<cdot>(senderIn_stream_as_i\<cdot>port_as\<cdot>port_i) = port_as"
+lemma sender_get_stream_as_in_as_id[simp]: "sender_get_stream_as\<cdot>(senderIn_stream_as_i\<cdot>port_as\<cdot>port_i) = port_as"
   apply(auto simp add: sender_get_stream_as.rep_eq senderIn_stream_as_i_def ubclUnion_ubundle_def)
-  by (metis sender_get_stream_as.rep_eq sender_stream_as_id)
+  by (metis sender_get_stream_as.rep_eq sender_get_stream_as_id)
 
-lemma senderin_stream_as_i_i_id[simp]: "sender_get_stream_i\<cdot>(senderIn_stream_as_i\<cdot>port_as\<cdot>port_i) = port_i"
+lemma sender_get_stream_i_in_i_id[simp]: "sender_get_stream_i\<cdot>(senderIn_stream_as_i\<cdot>port_as\<cdot>port_i) = port_i"
   apply(auto simp add: sender_get_stream_i.rep_eq senderIn_stream_as_i_def ubclUnion_ubundle_def)
-  by (metis sender_get_stream_i.rep_eq sender_stream_i_id)
+  by (metis sender_get_stream_i.rep_eq sender_get_stream_i_id)
 
-lemma senderout_stream_ds_ds_id[simp]: "sender_get_stream_ds\<cdot>(senderOut_stream_ds\<cdot>port_ds) = port_ds"
+lemma sender_get_stream_ds_out_ds_id[simp]: "sender_get_stream_ds\<cdot>(senderOut_stream_ds\<cdot>port_ds) = port_ds"
   apply(auto simp add: sender_get_stream_ds.rep_eq senderOut_stream_ds_def ubclUnion_ubundle_def)
-  by (metis sender_get_stream_ds.rep_eq sender_stream_ds_id)
+  by (metis sender_get_stream_ds.rep_eq sender_get_stream_ds_id)
 
 
 subsection \<open>tsyn to SB to one-element stream\<close>
 
+subsubsection \<open>Intern\<close>
+
+lemma sender_get_stream_as_single[simp]: "sender_get_stream_as\<cdot>(sender_as x) = \<up>x"
+  sorry
+
+lemma sender_get_stream_i_single[simp]: "sender_get_stream_i\<cdot>(sender_i x) = \<up>x"
+  sorry
+
+lemma sender_get_stream_ds_single[simp]: "sender_get_stream_ds\<cdot>(sender_ds x) = \<up>x"
+  sorry
+
+
 subsubsection \<open>In/Out\<close>
 
-lemma senderin_as_i_as_id[simp]: "sender_get_stream_as\<cdot>(senderIn_as_i port_as port_i) = \<up>port_as"
+lemma sender_get_stream_as_single_in_as_id[simp]: "sender_get_stream_as\<cdot>(senderIn_as_i port_as port_i) = \<up>port_as"
   apply(simp add: sender_get_stream_as_def senderIn_as_i_def)
   apply(subst sbe2sb_getch)
   apply(auto simp add: senderDom_def senderElemIn_as_i_def)
@@ -627,7 +674,7 @@ lemma senderin_as_i_as_id[simp]: "sender_get_stream_as\<cdot>(senderIn_as_i port
   apply(simp add: inj_def)
   by(simp add: sbeNull.rep_eq)
 
-lemma senderin_as_i_i_id[simp]: "sender_get_stream_i\<cdot>(senderIn_as_i port_as port_i) = \<up>port_i"
+lemma sender_get_stream_i_single_in_i_id[simp]: "sender_get_stream_i\<cdot>(senderIn_as_i port_as port_i) = \<up>port_i"
   apply(simp add: sender_get_stream_i_def senderIn_as_i_def)
   apply(subst sbe2sb_getch)
   apply(auto simp add: senderDom_def senderElemIn_as_i_def)
@@ -637,7 +684,7 @@ lemma senderin_as_i_i_id[simp]: "sender_get_stream_i\<cdot>(senderIn_as_i port_a
   apply(simp add: inj_def)
   by(simp add: sbeNull.rep_eq)
 
-lemma senderout_ds_ds_id[simp]: "sender_get_stream_ds\<cdot>(senderOut_ds port_ds) = \<up>port_ds"
+lemma sender_get_stream_ds_single_out_ds_id[simp]: "sender_get_stream_ds\<cdot>(senderOut_ds port_ds) = \<up>port_ds"
   apply(simp add: sender_get_stream_ds_def senderOut_ds_def)
   apply(subst sbe2sb_getch)
   apply(auto simp add: senderDom_def senderElemOut_ds_def)
@@ -646,6 +693,28 @@ lemma senderout_ds_ds_id[simp]: "sender_get_stream_ds\<cdot>(senderOut_ds port_d
   unfolding senderElem_get_ds_def senderElem_raw_ds.rep_eq
   apply(simp add: inj_def)
   by(simp add: sbeNull.rep_eq)
+
+
+section \<open>More Setter-Lemmas\<close>
+
+subsection \<open>SB to stream\<close>
+
+subsubsection \<open>Intern\<close>
+
+lemma sender_stream_as_conc:
+  "sender_stream_as\<cdot>(\<up>elem \<bullet> s) = ubConc (sender_as elem)\<cdot>(sender_stream_as\<cdot>s)"
+  apply (rule sender_get_stream_as_eq)
+  by simp_all
+
+lemma sender_stream_i_conc:
+  "sender_stream_i\<cdot>(\<up>elem \<bullet> s) = ubConc (sender_i elem)\<cdot>(sender_stream_i\<cdot>s)"
+  apply (rule sender_get_stream_i_eq)
+  by simp_all
+
+lemma sender_stream_ds_conc:
+  "sender_stream_ds\<cdot>(\<up>elem \<bullet> s) = ubConc (sender_ds elem)\<cdot>(sender_stream_ds\<cdot>s)"
+  apply (rule sender_get_stream_ds_eq)
+  by simp_all
 
 
 section \<open>Step-wise lemmata for the transition function\<close>
